<http://www.coypu.org/ontologies/em-dat/> <http://www.w3.org/1999/02/22-rdf-syntax-ns#type> <http://www.w3.org/2002/07/owl#Ontology> .
<http://www.coypu.org/ontologies/em-dat/Air> <http://www.w3.org/1999/02/22-rdf-syntax-ns#type> <http://www.w3.org/2002/07/owl#Class> .
<http://www.coypu.org/ontologies/em-dat/TransportAccident> <http://www.w3.org/1999/02/22-rdf-syntax-ns#type> <http://www.w3.org/2002/07/owl#Class> .
<http://www.coypu.org/ontologies/em-dat/Airburst> <http://www.w3.org/1999/02/22-rdf-syntax-ns#type> <http://www.w3.org/2002/07/owl#Class> .
<http://www.coypu.org/ontologies/em-dat/Impact> <http://www.w3.org/1999/02/22-rdf-syntax-ns#type> <http://www.w3.org/2002/07/owl#Class> .
<http://www.coypu.org/ontologies/em-dat/AnimalAccident> <http://www.w3.org/1999/02/22-rdf-syntax-ns#type> <http://www.w3.org/2002/07/owl#Class> .
<http://www.coypu.org/ontologies/em-dat/BiologicalDisaster> <http://www.w3.org/1999/02/22-rdf-syntax-ns#type> <http://www.w3.org/2002/07/owl#Class> .
<http://www.coypu.org/ontologies/em-dat/AshFall> <http://www.w3.org/1999/02/22-rdf-syntax-ns#type> <http://www.w3.org/2002/07/owl#Class> .
<http://www.coypu.org/ontologies/em-dat/VolcanicActivity> <http://www.w3.org/1999/02/22-rdf-syntax-ns#type> <http://www.w3.org/2002/07/owl#Class> .
<http://www.coypu.org/ontologies/em-dat/Avalanche> <http://www.w3.org/1999/02/22-rdf-syntax-ns#type> <http://www.w3.org/2002/07/owl#Class> .
<http://www.coypu.org/ontologies/em-dat/Landslide(wet)> <http://www.w3.org/1999/02/22-rdf-syntax-ns#type> <http://www.w3.org/2002/07/owl#Class> .
<http://www.coypu.org/ontologies/em-dat/Bacterial_Disease> <http://www.w3.org/1999/02/22-rdf-syntax-ns#type> <http://www.w3.org/2002/07/owl#Class> .
<http://www.coypu.org/ontologies/em-dat/Epidemic> <http://www.w3.org/1999/02/22-rdf-syntax-ns#type> <http://www.w3.org/2002/07/owl#Class> .
<http://www.coypu.org/ontologies/em-dat/NaturalDisaster> <http://www.w3.org/1999/02/22-rdf-syntax-ns#type> <http://www.w3.org/2002/07/owl#Class> .
<http://www.coypu.org/ontologies/em-dat/ChemicalSpill> <http://www.w3.org/1999/02/22-rdf-syntax-ns#type> <http://www.w3.org/2002/07/owl#Class> .
<http://www.coypu.org/ontologies/em-dat/IndustrialAccident> <http://www.w3.org/1999/02/22-rdf-syntax-ns#type> <http://www.w3.org/2002/07/owl#Class> .
<http://www.coypu.org/ontologies/em-dat/ClimatologicalDisaster> <http://www.w3.org/1999/02/22-rdf-syntax-ns#type> <http://www.w3.org/2002/07/owl#Class> .
<http://www.coypu.org/ontologies/em-dat/CoastalFlood> <http://www.w3.org/1999/02/22-rdf-syntax-ns#type> <http://www.w3.org/2002/07/owl#Class> .
<http://www.coypu.org/ontologies/em-dat/Flood> <http://www.w3.org/1999/02/22-rdf-syntax-ns#type> <http://www.w3.org/2002/07/owl#Class> .
<http://www.coypu.org/ontologies/em-dat/ColdWave> <http://www.w3.org/1999/02/22-rdf-syntax-ns#type> <http://www.w3.org/2002/07/owl#Class> .
<http://www.coypu.org/ontologies/em-dat/ExtremeTemperature> <http://www.w3.org/1999/02/22-rdf-syntax-ns#type> <http://www.w3.org/2002/07/owl#Class> .
<http://www.coypu.org/ontologies/em-dat/Collapse> <http://www.w3.org/1999/02/22-rdf-syntax-ns#type> <http://www.w3.org/2002/07/owl#Class> .
<http://www.coypu.org/ontologies/em-dat/MiscelleanousAccident> <http://www.w3.org/1999/02/22-rdf-syntax-ns#type> <http://www.w3.org/2002/07/owl#Class> .
<http://www.coypu.org/ontologies/em-dat/ConvectiveStorm> <http://www.w3.org/1999/02/22-rdf-syntax-ns#type> <http://www.w3.org/2002/07/owl#Class> .
<http://www.coypu.org/ontologies/em-dat/Storm> <http://www.w3.org/1999/02/22-rdf-syntax-ns#type> <http://www.w3.org/2002/07/owl#Class> .
<http://www.coypu.org/ontologies/em-dat/Derecho> <http://www.w3.org/1999/02/22-rdf-syntax-ns#type> <http://www.w3.org/2002/07/owl#Class> .
<http://www.coypu.org/ontologies/em-dat/Disaster> <http://www.w3.org/1999/02/22-rdf-syntax-ns#type> <http://www.w3.org/2002/07/owl#Class> .
<http://www.coypu.org/ontologies/em-dat/Drought> <http://www.w3.org/1999/02/22-rdf-syntax-ns#type> <http://www.w3.org/2002/07/owl#Class> .
<http://www.coypu.org/ontologies/em-dat/Earthquake> <http://www.w3.org/1999/02/22-rdf-syntax-ns#type> <http://www.w3.org/2002/07/owl#Class> .
<http://www.coypu.org/ontologies/em-dat/GeophysicalDisaster> <http://www.w3.org/1999/02/22-rdf-syntax-ns#type> <http://www.w3.org/2002/07/owl#Class> .
<http://www.coypu.org/ontologies/em-dat/EnergeticParticles> <http://www.w3.org/1999/02/22-rdf-syntax-ns#type> <http://www.w3.org/2002/07/owl#Class> .
<http://www.coypu.org/ontologies/em-dat/SpaceWeather> <http://www.w3.org/1999/02/22-rdf-syntax-ns#type> <http://www.w3.org/2002/07/owl#Class> .
<http://www.coypu.org/ontologies/em-dat/Explosion> <http://www.w3.org/1999/02/22-rdf-syntax-ns#type> <http://www.w3.org/2002/07/owl#Class> .
<http://www.coypu.org/ontologies/em-dat/ExtraTropicalStorm> <http://www.w3.org/1999/02/22-rdf-syntax-ns#type> <http://www.w3.org/2002/07/owl#Class> .
<http://www.coypu.org/ontologies/em-dat/ExtraterrestrialDisaster> <http://www.w3.org/1999/02/22-rdf-syntax-ns#type> <http://www.w3.org/2002/07/owl#Class> .
<http://www.coypu.org/ontologies/em-dat/MeteorologicalDisaster> <http://www.w3.org/1999/02/22-rdf-syntax-ns#type> <http://www.w3.org/2002/07/owl#Class> .
<http://www.coypu.org/ontologies/em-dat/Fire> <http://www.w3.org/1999/02/22-rdf-syntax-ns#type> <http://www.w3.org/2002/07/owl#Class> .
<http://www.coypu.org/ontologies/em-dat/FlashFlood> <http://www.w3.org/1999/02/22-rdf-syntax-ns#type> <http://www.w3.org/2002/07/owl#Class> .
<http://www.coypu.org/ontologies/em-dat/HydrologicalDisaster> <http://www.w3.org/1999/02/22-rdf-syntax-ns#type> <http://www.w3.org/2002/07/owl#Class> .
<http://www.coypu.org/ontologies/em-dat/Fog> <http://www.w3.org/1999/02/22-rdf-syntax-ns#type> <http://www.w3.org/2002/07/owl#Class> .
<http://www.coypu.org/ontologies/em-dat/ForestFire> <http://www.w3.org/1999/02/22-rdf-syntax-ns#type> <http://www.w3.org/2002/07/owl#Class> .
<http://www.coypu.org/ontologies/em-dat/Wildfire> <http://www.w3.org/1999/02/22-rdf-syntax-ns#type> <http://www.w3.org/2002/07/owl#Class> .
<http://www.coypu.org/ontologies/em-dat/FrostOrFreeze> <http://www.w3.org/1999/02/22-rdf-syntax-ns#type> <http://www.w3.org/2002/07/owl#Class> .
<http://www.coypu.org/ontologies/em-dat/SevereWinterConditions> <http://www.w3.org/1999/02/22-rdf-syntax-ns#type> <http://www.w3.org/2002/07/owl#Class> .
<http://www.coypu.org/ontologies/em-dat/FungalDisease> <http://www.w3.org/1999/02/22-rdf-syntax-ns#type> <http://www.w3.org/2002/07/owl#Class> .
<http://www.coypu.org/ontologies/em-dat/GasLeak> <http://www.w3.org/1999/02/22-rdf-syntax-ns#type> <http://www.w3.org/2002/07/owl#Class> .
<http://www.coypu.org/ontologies/em-dat/GeomagneticStorm> <http://www.w3.org/1999/02/22-rdf-syntax-ns#type> <http://www.w3.org/2002/07/owl#Class> .
<http://www.coypu.org/ontologies/em-dat/GlacialLakeOutburst> <http://www.w3.org/1999/02/22-rdf-syntax-ns#type> <http://www.w3.org/2002/07/owl#Class> .
<http://www.coypu.org/ontologies/em-dat/Grasshopper> <http://www.w3.org/1999/02/22-rdf-syntax-ns#type> <http://www.w3.org/2002/07/owl#Class> .
<http://www.coypu.org/ontologies/em-dat/InsectInfestation> <http://www.w3.org/1999/02/22-rdf-syntax-ns#type> <http://www.w3.org/2002/07/owl#Class> .
<http://www.coypu.org/ontologies/em-dat/GroundMovement> <http://www.w3.org/1999/02/22-rdf-syntax-ns#type> <http://www.w3.org/2002/07/owl#Class> .
<http://www.coypu.org/ontologies/em-dat/Hail> <http://www.w3.org/1999/02/22-rdf-syntax-ns#type> <http://www.w3.org/2002/07/owl#Class> .
<http://www.coypu.org/ontologies/em-dat/HeatWave> <http://www.w3.org/1999/02/22-rdf-syntax-ns#type> <http://www.w3.org/2002/07/owl#Class> .
<http://www.coypu.org/ontologies/em-dat/IceJamFlood> <http://www.w3.org/1999/02/22-rdf-syntax-ns#type> <http://www.w3.org/2002/07/owl#Class> .
<http://www.coypu.org/ontologies/em-dat/TechnologicalDisaster> <http://www.w3.org/1999/02/22-rdf-syntax-ns#type> <http://www.w3.org/2002/07/owl#Class> .
<http://www.coypu.org/ontologies/em-dat/Lahar> <http://www.w3.org/1999/02/22-rdf-syntax-ns#type> <http://www.w3.org/2002/07/owl#Class> .
<http://www.coypu.org/ontologies/em-dat/LandFire> <http://www.w3.org/1999/02/22-rdf-syntax-ns#type> <http://www.w3.org/2002/07/owl#Class> .
<http://www.coypu.org/ontologies/em-dat/LavaFlow> <http://www.w3.org/1999/02/22-rdf-syntax-ns#type> <http://www.w3.org/2002/07/owl#Class> .
<http://www.coypu.org/ontologies/em-dat/LightningOrThunderstorm> <http://www.w3.org/1999/02/22-rdf-syntax-ns#type> <http://www.w3.org/2002/07/owl#Class> .
<http://www.coypu.org/ontologies/em-dat/Locust> <http://www.w3.org/1999/02/22-rdf-syntax-ns#type> <http://www.w3.org/2002/07/owl#Class> .
<http://www.coypu.org/ontologies/em-dat/OilSpill> <http://www.w3.org/1999/02/22-rdf-syntax-ns#type> <http://www.w3.org/2002/07/owl#Class> .
<http://www.coypu.org/ontologies/em-dat/Other> <http://www.w3.org/1999/02/22-rdf-syntax-ns#type> <http://www.w3.org/2002/07/owl#Class> .
<http://www.coypu.org/ontologies/em-dat/ParasiticDisease> <http://www.w3.org/1999/02/22-rdf-syntax-ns#type> <http://www.w3.org/2002/07/owl#Class> .
<http://www.coypu.org/ontologies/em-dat/Poisoning> <http://www.w3.org/1999/02/22-rdf-syntax-ns#type> <http://www.w3.org/2002/07/owl#Class> .
<http://www.coypu.org/ontologies/em-dat/PrionDisease> <http://www.w3.org/1999/02/22-rdf-syntax-ns#type> <http://www.w3.org/2002/07/owl#Class> .
<http://www.coypu.org/ontologies/em-dat/PyroclasticFlow> <http://www.w3.org/1999/02/22-rdf-syntax-ns#type> <http://www.w3.org/2002/07/owl#Class> .
<http://www.coypu.org/ontologies/em-dat/Radiation> <http://www.w3.org/1999/02/22-rdf-syntax-ns#type> <http://www.w3.org/2002/07/owl#Class> .
<http://www.coypu.org/ontologies/em-dat/Rail> <http://www.w3.org/1999/02/22-rdf-syntax-ns#type> <http://www.w3.org/2002/07/owl#Class> .
<http://www.coypu.org/ontologies/em-dat/Rain> <http://www.w3.org/1999/02/22-rdf-syntax-ns#type> <http://www.w3.org/2002/07/owl#Class> .
<http://www.coypu.org/ontologies/em-dat/RiverineFlood> <http://www.w3.org/1999/02/22-rdf-syntax-ns#type> <http://www.w3.org/2002/07/owl#Class> .
<http://www.coypu.org/ontologies/em-dat/Road> <http://www.w3.org/1999/02/22-rdf-syntax-ns#type> <http://www.w3.org/2002/07/owl#Class> .
<http://www.coypu.org/ontologies/em-dat/RockFall> <http://www.w3.org/1999/02/22-rdf-syntax-ns#type> <http://www.w3.org/2002/07/owl#Class> .
<http://www.coypu.org/ontologies/em-dat/MassMovement_(dry)> <http://www.w3.org/1999/02/22-rdf-syntax-ns#type> <http://www.w3.org/2002/07/owl#Class> .
<http://www.coypu.org/ontologies/em-dat/RogueWave> <http://www.w3.org/1999/02/22-rdf-syntax-ns#type> <http://www.w3.org/2002/07/owl#Class> .
<http://www.coypu.org/ontologies/em-dat/WaveAction> <http://www.w3.org/1999/02/22-rdf-syntax-ns#type> <http://www.w3.org/2002/07/owl#Class> .
<http://www.coypu.org/ontologies/em-dat/SandOrDustStorm> <http://www.w3.org/1999/02/22-rdf-syntax-ns#type> <http://www.w3.org/2002/07/owl#Class> .
<http://www.coypu.org/ontologies/em-dat/Seiche> <http://www.w3.org/1999/02/22-rdf-syntax-ns#type> <http://www.w3.org/2002/07/owl#Class> .
<http://www.coypu.org/ontologies/em-dat/SevereStorm> <http://www.w3.org/1999/02/22-rdf-syntax-ns#type> <http://www.w3.org/2002/07/owl#Class> .
<http://www.coypu.org/ontologies/em-dat/Shockwave> <http://www.w3.org/1999/02/22-rdf-syntax-ns#type> <http://www.w3.org/2002/07/owl#Class> .
<http://www.coypu.org/ontologies/em-dat/SnowOrIce> <http://www.w3.org/1999/02/22-rdf-syntax-ns#type> <http://www.w3.org/2002/07/owl#Class> .
<http://www.coypu.org/ontologies/em-dat/StormOrSurge> <http://www.w3.org/1999/02/22-rdf-syntax-ns#type> <http://www.w3.org/2002/07/owl#Class> .
<http://www.coypu.org/ontologies/em-dat/Tornado> <http://www.w3.org/1999/02/22-rdf-syntax-ns#type> <http://www.w3.org/2002/07/owl#Class> .
<http://www.coypu.org/ontologies/em-dat/TropicalStorm> <http://www.w3.org/1999/02/22-rdf-syntax-ns#type> <http://www.w3.org/2002/07/owl#Class> .
<http://www.coypu.org/ontologies/em-dat/Tsunami> <http://www.w3.org/1999/02/22-rdf-syntax-ns#type> <http://www.w3.org/2002/07/owl#Class> .
<http://www.coypu.org/ontologies/em-dat/ViralDisease> <http://www.w3.org/1999/02/22-rdf-syntax-ns#type> <http://www.w3.org/2002/07/owl#Class> .
<http://www.coypu.org/ontologies/em-dat/Water> <http://www.w3.org/1999/02/22-rdf-syntax-ns#type> <http://www.w3.org/2002/07/owl#Class> .
<http://www.coypu.org/ontologies/em-dat/Wind> <http://www.w3.org/1999/02/22-rdf-syntax-ns#type> <http://www.w3.org/2002/07/owl#Class> .
<http://www.coypu.org/ontologies/em-dat/WinterStormOrBlizzard> <http://www.w3.org/1999/02/22-rdf-syntax-ns#type> <http://www.w3.org/2002/07/owl#Class> .
<http://www.coypu.org/ontologies/em-dat/Landslide(dry)> <http://www.w3.org/1999/02/22-rdf-syntax-ns#type> <http://www.w3.org/2002/07/owl#Class> .
_:node806 <http://www.w3.org/1999/02/22-rdf-syntax-ns#type> <http://www.w3.org/2002/07/owl#Class> .
_:node809 <http://www.w3.org/1999/02/22-rdf-syntax-ns#type> <http://www.w3.org/2002/07/owl#Class> .
_:node812 <http://www.w3.org/1999/02/22-rdf-syntax-ns#type> <http://www.w3.org/2002/07/owl#Class> .
_:node815 <http://www.w3.org/1999/02/22-rdf-syntax-ns#type> <http://www.w3.org/2002/07/owl#Class> .
<http://www.coypu.org/ontologies/em-dat/Air> <http://www.w3.org/2000/01/rdf-schema#subClassOf> <http://www.coypu.org/ontologies/em-dat/TransportAccident> .
<http://www.coypu.org/ontologies/em-dat/TransportAccident> <http://www.w3.org/2000/01/rdf-schema#subClassOf> <http://www.coypu.org/ontologies/em-dat/TechnologicalDisaster> .
<http://www.coypu.org/ontologies/em-dat/Airburst> <http://www.w3.org/2000/01/rdf-schema#subClassOf> <http://www.coypu.org/ontologies/em-dat/Impact> .
<http://www.coypu.org/ontologies/em-dat/Impact> <http://www.w3.org/2000/01/rdf-schema#subClassOf> <http://www.coypu.org/ontologies/em-dat/ExtraterrestrialDisaster> .
<http://www.coypu.org/ontologies/em-dat/AnimalAccident> <http://www.w3.org/2000/01/rdf-schema#subClassOf> <http://www.coypu.org/ontologies/em-dat/BiologicalDisaster> .
<http://www.coypu.org/ontologies/em-dat/BiologicalDisaster> <http://www.w3.org/2000/01/rdf-schema#subClassOf> <http://www.coypu.org/ontologies/em-dat/NaturalDisaster> .
<http://www.coypu.org/ontologies/em-dat/AshFall> <http://www.w3.org/2000/01/rdf-schema#subClassOf> <http://www.coypu.org/ontologies/em-dat/VolcanicActivity> .
<http://www.coypu.org/ontologies/em-dat/VolcanicActivity> <http://www.w3.org/2000/01/rdf-schema#subClassOf> <http://www.coypu.org/ontologies/em-dat/GeophysicalDisaster> .
<http://www.coypu.org/ontologies/em-dat/Avalanche> <http://www.w3.org/2000/01/rdf-schema#subClassOf> <http://www.coypu.org/ontologies/em-dat/Landslide(wet)> .
<http://www.coypu.org/ontologies/em-dat/Landslide(wet)> <http://www.w3.org/2000/01/rdf-schema#subClassOf> <http://www.coypu.org/ontologies/em-dat/HydrologicalDisaster> .
<http://www.coypu.org/ontologies/em-dat/Bacterial_Disease> <http://www.w3.org/2000/01/rdf-schema#subClassOf> <http://www.coypu.org/ontologies/em-dat/Epidemic> .
<http://www.coypu.org/ontologies/em-dat/Epidemic> <http://www.w3.org/2000/01/rdf-schema#subClassOf> <http://www.coypu.org/ontologies/em-dat/BiologicalDisaster> .
<http://www.coypu.org/ontologies/em-dat/NaturalDisaster> <http://www.w3.org/2000/01/rdf-schema#subClassOf> <http://www.coypu.org/ontologies/em-dat/Disaster> .
<http://www.coypu.org/ontologies/em-dat/ChemicalSpill> <http://www.w3.org/2000/01/rdf-schema#subClassOf> <http://www.coypu.org/ontologies/em-dat/IndustrialAccident> .
<http://www.coypu.org/ontologies/em-dat/IndustrialAccident> <http://www.w3.org/2000/01/rdf-schema#subClassOf> <http://www.coypu.org/ontologies/em-dat/TechnologicalDisaster> .
<http://www.coypu.org/ontologies/em-dat/ClimatologicalDisaster> <http://www.w3.org/2000/01/rdf-schema#subClassOf> <http://www.coypu.org/ontologies/em-dat/NaturalDisaster> .
<http://www.coypu.org/ontologies/em-dat/CoastalFlood> <http://www.w3.org/2000/01/rdf-schema#subClassOf> <http://www.coypu.org/ontologies/em-dat/Flood> .
<http://www.coypu.org/ontologies/em-dat/Flood> <http://www.w3.org/2000/01/rdf-schema#subClassOf> <http://www.coypu.org/ontologies/em-dat/HydrologicalDisaster> .
<http://www.coypu.org/ontologies/em-dat/ColdWave> <http://www.w3.org/2000/01/rdf-schema#subClassOf> <http://www.coypu.org/ontologies/em-dat/ExtremeTemperature> .
<http://www.coypu.org/ontologies/em-dat/ExtremeTemperature> <http://www.w3.org/2000/01/rdf-schema#subClassOf> <http://www.coypu.org/ontologies/em-dat/MeteorologicalDisaster> .
<http://www.coypu.org/ontologies/em-dat/Collapse> <http://www.w3.org/2000/01/rdf-schema#subClassOf> _:node806 .
<http://www.coypu.org/ontologies/em-dat/MiscelleanousAccident> <http://www.w3.org/2000/01/rdf-schema#subClassOf> <http://www.coypu.org/ontologies/em-dat/TechnologicalDisaster> .
<http://www.coypu.org/ontologies/em-dat/ConvectiveStorm> <http://www.w3.org/2000/01/rdf-schema#subClassOf> <http://www.coypu.org/ontologies/em-dat/Storm> .
<http://www.coypu.org/ontologies/em-dat/Storm> <http://www.w3.org/2000/01/rdf-schema#subClassOf> <http://www.coypu.org/ontologies/em-dat/MeteorologicalDisaster> .
<http://www.coypu.org/ontologies/em-dat/Derecho> <http://www.w3.org/2000/01/rdf-schema#subClassOf> <http://www.coypu.org/ontologies/em-dat/ConvectiveStorm> .
<http://www.coypu.org/ontologies/em-dat/Drought> <http://www.w3.org/2000/01/rdf-schema#subClassOf> <http://www.coypu.org/ontologies/em-dat/ClimatologicalDisaster> .
<http://www.coypu.org/ontologies/em-dat/Earthquake> <http://www.w3.org/2000/01/rdf-schema#subClassOf> <http://www.coypu.org/ontologies/em-dat/GeophysicalDisaster> .
<http://www.coypu.org/ontologies/em-dat/GeophysicalDisaster> <http://www.w3.org/2000/01/rdf-schema#subClassOf> <http://www.coypu.org/ontologies/em-dat/NaturalDisaster> .
<http://www.coypu.org/ontologies/em-dat/EnergeticParticles> <http://www.w3.org/2000/01/rdf-schema#subClassOf> <http://www.coypu.org/ontologies/em-dat/SpaceWeather> .
<http://www.coypu.org/ontologies/em-dat/SpaceWeather> <http://www.w3.org/2000/01/rdf-schema#subClassOf> <http://www.coypu.org/ontologies/em-dat/ExtraterrestrialDisaster> .
<http://www.coypu.org/ontologies/em-dat/Explosion> <http://www.w3.org/2000/01/rdf-schema#subClassOf> _:node809 .
<http://www.coypu.org/ontologies/em-dat/ExtraTropicalStorm> <http://www.w3.org/2000/01/rdf-schema#subClassOf> <http://www.coypu.org/ontologies/em-dat/Storm> .
<http://www.coypu.org/ontologies/em-dat/ExtraterrestrialDisaster> <http://www.w3.org/2000/01/rdf-schema#subClassOf> <http://www.coypu.org/ontologies/em-dat/NaturalDisaster> .
<http://www.coypu.org/ontologies/em-dat/MeteorologicalDisaster> <http://www.w3.org/2000/01/rdf-schema#subClassOf> <http://www.coypu.org/ontologies/em-dat/NaturalDisaster> .
<http://www.coypu.org/ontologies/em-dat/Fire> <http://www.w3.org/2000/01/rdf-schema#subClassOf> _:node812 .
<http://www.coypu.org/ontologies/em-dat/FlashFlood> <http://www.w3.org/2000/01/rdf-schema#subClassOf> <http://www.coypu.org/ontologies/em-dat/Flood> .
<http://www.coypu.org/ontologies/em-dat/HydrologicalDisaster> <http://www.w3.org/2000/01/rdf-schema#subClassOf> <http://www.coypu.org/ontologies/em-dat/NaturalDisaster> .
<http://www.coypu.org/ontologies/em-dat/Fog> <http://www.w3.org/2000/01/rdf-schema#subClassOf> <http://www.coypu.org/ontologies/em-dat/MeteorologicalDisaster> .
<http://www.coypu.org/ontologies/em-dat/ForestFire> <http://www.w3.org/2000/01/rdf-schema#subClassOf> <http://www.coypu.org/ontologies/em-dat/Wildfire> .
<http://www.coypu.org/ontologies/em-dat/Wildfire> <http://www.w3.org/2000/01/rdf-schema#subClassOf> <http://www.coypu.org/ontologies/em-dat/ClimatologicalDisaster> .
<http://www.coypu.org/ontologies/em-dat/FrostOrFreeze> <http://www.w3.org/2000/01/rdf-schema#subClassOf> <http://www.coypu.org/ontologies/em-dat/SevereWinterConditions> .
<http://www.coypu.org/ontologies/em-dat/SevereWinterConditions> <http://www.w3.org/2000/01/rdf-schema#subClassOf> <http://www.coypu.org/ontologies/em-dat/ExtremeTemperature> .
<http://www.coypu.org/ontologies/em-dat/FungalDisease> <http://www.w3.org/2000/01/rdf-schema#subClassOf> <http://www.coypu.org/ontologies/em-dat/Epidemic> .
<http://www.coypu.org/ontologies/em-dat/GasLeak> <http://www.w3.org/2000/01/rdf-schema#subClassOf> <http://www.coypu.org/ontologies/em-dat/IndustrialAccident> .
<http://www.coypu.org/ontologies/em-dat/GeomagneticStorm> <http://www.w3.org/2000/01/rdf-schema#subClassOf> <http://www.coypu.org/ontologies/em-dat/SpaceWeather> .
<http://www.coypu.org/ontologies/em-dat/GlacialLakeOutburst> <http://www.w3.org/2000/01/rdf-schema#subClassOf> <http://www.coypu.org/ontologies/em-dat/ClimatologicalDisaster> .
<http://www.coypu.org/ontologies/em-dat/Grasshopper> <http://www.w3.org/2000/01/rdf-schema#subClassOf> <http://www.coypu.org/ontologies/em-dat/InsectInfestation> .
<http://www.coypu.org/ontologies/em-dat/InsectInfestation> <http://www.w3.org/2000/01/rdf-schema#subClassOf> <http://www.coypu.org/ontologies/em-dat/BiologicalDisaster> .
<http://www.coypu.org/ontologies/em-dat/GroundMovement> <http://www.w3.org/2000/01/rdf-schema#subClassOf> <http://www.coypu.org/ontologies/em-dat/Earthquake> .
<http://www.coypu.org/ontologies/em-dat/Hail> <http://www.w3.org/2000/01/rdf-schema#subClassOf> <http://www.coypu.org/ontologies/em-dat/ConvectiveStorm> .
<http://www.coypu.org/ontologies/em-dat/HeatWave> <http://www.w3.org/2000/01/rdf-schema#subClassOf> <http://www.coypu.org/ontologies/em-dat/ExtremeTemperature> .
<http://www.coypu.org/ontologies/em-dat/IceJamFlood> <http://www.w3.org/2000/01/rdf-schema#subClassOf> <http://www.coypu.org/ontologies/em-dat/Flood> .
<http://www.coypu.org/ontologies/em-dat/TechnologicalDisaster> <http://www.w3.org/2000/01/rdf-schema#subClassOf> <http://www.coypu.org/ontologies/em-dat/Disaster> .
<http://www.coypu.org/ontologies/em-dat/Lahar> <http://www.w3.org/2000/01/rdf-schema#subClassOf> <http://www.coypu.org/ontologies/em-dat/VolcanicActivity> .
<http://www.coypu.org/ontologies/em-dat/LandFire> <http://www.w3.org/2000/01/rdf-schema#subClassOf> <http://www.coypu.org/ontologies/em-dat/Wildfire> .
<http://www.coypu.org/ontologies/em-dat/LavaFlow> <http://www.w3.org/2000/01/rdf-schema#subClassOf> <http://www.coypu.org/ontologies/em-dat/VolcanicActivity> .
<http://www.coypu.org/ontologies/em-dat/LightningOrThunderstorm> <http://www.w3.org/2000/01/rdf-schema#subClassOf> <http://www.coypu.org/ontologies/em-dat/ConvectiveStorm> .
<http://www.coypu.org/ontologies/em-dat/Locust> <http://www.w3.org/2000/01/rdf-schema#subClassOf> <http://www.coypu.org/ontologies/em-dat/InsectInfestation> .
<http://www.coypu.org/ontologies/em-dat/OilSpill> <http://www.w3.org/2000/01/rdf-schema#subClassOf> <http://www.coypu.org/ontologies/em-dat/IndustrialAccident> .
<http://www.coypu.org/ontologies/em-dat/Other> <http://www.w3.org/2000/01/rdf-schema#subClassOf> _:node815 .
<http://www.coypu.org/ontologies/em-dat/ParasiticDisease> <http://www.w3.org/2000/01/rdf-schema#subClassOf> <http://www.coypu.org/ontologies/em-dat/Epidemic> .
<http://www.coypu.org/ontologies/em-dat/Poisoning> <http://www.w3.org/2000/01/rdf-schema#subClassOf> <http://www.coypu.org/ontologies/em-dat/IndustrialAccident> .
<http://www.coypu.org/ontologies/em-dat/PrionDisease> <http://www.w3.org/2000/01/rdf-schema#subClassOf> <http://www.coypu.org/ontologies/em-dat/Epidemic> .
<http://www.coypu.org/ontologies/em-dat/PyroclasticFlow> <http://www.w3.org/2000/01/rdf-schema#subClassOf> <http://www.coypu.org/ontologies/em-dat/VolcanicActivity> .
<http://www.coypu.org/ontologies/em-dat/Radiation> <http://www.w3.org/2000/01/rdf-schema#subClassOf> <http://www.coypu.org/ontologies/em-dat/IndustrialAccident> .
<http://www.coypu.org/ontologies/em-dat/Rail> <http://www.w3.org/2000/01/rdf-schema#subClassOf> <http://www.coypu.org/ontologies/em-dat/TransportAccident> .
<http://www.coypu.org/ontologies/em-dat/Rain> <http://www.w3.org/2000/01/rdf-schema#subClassOf> <http://www.coypu.org/ontologies/em-dat/ConvectiveStorm> .
<http://www.coypu.org/ontologies/em-dat/RiverineFlood> <http://www.w3.org/2000/01/rdf-schema#subClassOf> <http://www.coypu.org/ontologies/em-dat/Flood> .
<http://www.coypu.org/ontologies/em-dat/Road> <http://www.w3.org/2000/01/rdf-schema#subClassOf> <http://www.coypu.org/ontologies/em-dat/TransportAccident> .
<http://www.coypu.org/ontologies/em-dat/RockFall> <http://www.w3.org/2000/01/rdf-schema#subClassOf> <http://www.coypu.org/ontologies/em-dat/MassMovement_(dry)> .
<http://www.coypu.org/ontologies/em-dat/MassMovement_(dry)> <http://www.w3.org/2000/01/rdf-schema#subClassOf> <http://www.coypu.org/ontologies/em-dat/GeophysicalDisaster> .
<http://www.coypu.org/ontologies/em-dat/RogueWave> <http://www.w3.org/2000/01/rdf-schema#subClassOf> <http://www.coypu.org/ontologies/em-dat/WaveAction> .
<http://www.coypu.org/ontologies/em-dat/WaveAction> <http://www.w3.org/2000/01/rdf-schema#subClassOf> <http://www.coypu.org/ontologies/em-dat/HydrologicalDisaster> .
<http://www.coypu.org/ontologies/em-dat/SandOrDustStorm> <http://www.w3.org/2000/01/rdf-schema#subClassOf> <http://www.coypu.org/ontologies/em-dat/ConvectiveStorm> .
<http://www.coypu.org/ontologies/em-dat/Seiche> <http://www.w3.org/2000/01/rdf-schema#subClassOf> <http://www.coypu.org/ontologies/em-dat/WaveAction> .
<http://www.coypu.org/ontologies/em-dat/SevereStorm> <http://www.w3.org/2000/01/rdf-schema#subClassOf> <http://www.coypu.org/ontologies/em-dat/ConvectiveStorm> .
<http://www.coypu.org/ontologies/em-dat/Shockwave> <http://www.w3.org/2000/01/rdf-schema#subClassOf> <http://www.coypu.org/ontologies/em-dat/SpaceWeather> .
<http://www.coypu.org/ontologies/em-dat/SnowOrIce> <http://www.w3.org/2000/01/rdf-schema#subClassOf> <http://www.coypu.org/ontologies/em-dat/SevereWinterConditions> .
<http://www.coypu.org/ontologies/em-dat/StormOrSurge> <http://www.w3.org/2000/01/rdf-schema#subClassOf> <http://www.coypu.org/ontologies/em-dat/ConvectiveStorm> .
<http://www.coypu.org/ontologies/em-dat/Tornado> <http://www.w3.org/2000/01/rdf-schema#subClassOf> <http://www.coypu.org/ontologies/em-dat/ConvectiveStorm> .
<http://www.coypu.org/ontologies/em-dat/TropicalStorm> <http://www.w3.org/2000/01/rdf-schema#subClassOf> <http://www.coypu.org/ontologies/em-dat/Storm> .
<http://www.coypu.org/ontologies/em-dat/Tsunami> <http://www.w3.org/2000/01/rdf-schema#subClassOf> <http://www.coypu.org/ontologies/em-dat/Earthquake> .
<http://www.coypu.org/ontologies/em-dat/ViralDisease> <http://www.w3.org/2000/01/rdf-schema#subClassOf> <http://www.coypu.org/ontologies/em-dat/Epidemic> .
<http://www.coypu.org/ontologies/em-dat/Water> <http://www.w3.org/2000/01/rdf-schema#subClassOf> <http://www.coypu.org/ontologies/em-dat/TransportAccident> .
<http://www.coypu.org/ontologies/em-dat/Wind> <http://www.w3.org/2000/01/rdf-schema#subClassOf> <http://www.coypu.org/ontologies/em-dat/ConvectiveStorm> .
<http://www.coypu.org/ontologies/em-dat/WinterStormOrBlizzard> <http://www.w3.org/2000/01/rdf-schema#subClassOf> <http://www.coypu.org/ontologies/em-dat/ConvectiveStorm> .
<http://www.coypu.org/ontologies/em-dat/Landslide(dry)> <http://www.w3.org/2000/01/rdf-schema#subClassOf> <http://www.coypu.org/ontologies/em-dat/MassMovement_(dry)> .
<http://www.coypu.org/ontologies/em-dat/> <http://www.w3.org/2000/01/rdf-schema#label> "emdat: Disaster Classification Ontology" .
<http://www.coypu.org/ontologies/em-dat/Air> <http://www.w3.org/2000/01/rdf-schema#label> "air"@en .
<http://www.coypu.org/ontologies/em-dat/TransportAccident> <http://www.w3.org/2000/01/rdf-schema#label> "transport accident"@en .
<http://www.coypu.org/ontologies/em-dat/Airburst> <http://www.w3.org/2000/01/rdf-schema#label> "airburst"@en .
<http://www.coypu.org/ontologies/em-dat/Impact> <http://www.w3.org/2000/01/rdf-schema#label> "impact"@en .
<http://www.coypu.org/ontologies/em-dat/AnimalAccident> <http://www.w3.org/2000/01/rdf-schema#label> "animal accident"@en .
<http://www.coypu.org/ontologies/em-dat/BiologicalDisaster> <http://www.w3.org/2000/01/rdf-schema#label> "biological disaster"@en .
<http://www.coypu.org/ontologies/em-dat/AshFall> <http://www.w3.org/2000/01/rdf-schema#label> "ash fall"@en .
<http://www.coypu.org/ontologies/em-dat/VolcanicActivity> <http://www.w3.org/2000/01/rdf-schema#label> "volcanic activity"@en .
<http://www.coypu.org/ontologies/em-dat/Avalanche> <http://www.w3.org/2000/01/rdf-schema#label> "avalanche (snow, debris, mudflow, rockfall)"@en .
<http://www.coypu.org/ontologies/em-dat/Landslide(wet)> <http://www.w3.org/2000/01/rdf-schema#label> "landslide (wet)"@en .
<http://www.coypu.org/ontologies/em-dat/Bacterial_Disease> <http://www.w3.org/2000/01/rdf-schema#label> "bacterial disease"@en .
<http://www.coypu.org/ontologies/em-dat/Epidemic> <http://www.w3.org/2000/01/rdf-schema#label> "epidemic"@en .
<http://www.coypu.org/ontologies/em-dat/NaturalDisaster> <http://www.w3.org/2000/01/rdf-schema#label> "natural disaster"@en .
<http://www.coypu.org/ontologies/em-dat/ChemicalSpill> <http://www.w3.org/2000/01/rdf-schema#label> "chemical spill"@en .
<http://www.coypu.org/ontologies/em-dat/IndustrialAccident> <http://www.w3.org/2000/01/rdf-schema#label> "industrial accident"@en .
<http://www.coypu.org/ontologies/em-dat/ClimatologicalDisaster> <http://www.w3.org/2000/01/rdf-schema#label> "climatological disaster"@en .
<http://www.coypu.org/ontologies/em-dat/CoastalFlood> <http://www.w3.org/2000/01/rdf-schema#label> "coastal flood"@en .
<http://www.coypu.org/ontologies/em-dat/Flood> <http://www.w3.org/2000/01/rdf-schema#label> "flood"@en .
<http://www.coypu.org/ontologies/em-dat/ColdWave> <http://www.w3.org/2000/01/rdf-schema#label> "cold wave"@en .
<http://www.coypu.org/ontologies/em-dat/ExtremeTemperature> <http://www.w3.org/2000/01/rdf-schema#label> "extreme temperature"@en .
<http://www.coypu.org/ontologies/em-dat/Collapse> <http://www.w3.org/2000/01/rdf-schema#label> "collapse"@en .
<http://www.coypu.org/ontologies/em-dat/MiscelleanousAccident> <http://www.w3.org/2000/01/rdf-schema#label> "miscelleanous accident"@en .
<http://www.coypu.org/ontologies/em-dat/ConvectiveStorm> <http://www.w3.org/2000/01/rdf-schema#label> "convective storm"@en .
<http://www.coypu.org/ontologies/em-dat/Storm> <http://www.w3.org/2000/01/rdf-schema#label> "storm"@en .
<http://www.coypu.org/ontologies/em-dat/Derecho> <http://www.w3.org/2000/01/rdf-schema#label> "derecho"@en .
<http://www.coypu.org/ontologies/em-dat/Disaster> <http://www.w3.org/2000/01/rdf-schema#label> "disaster"@en .
<http://www.coypu.org/ontologies/em-dat/Drought> <http://www.w3.org/2000/01/rdf-schema#label> "drought"@en .
<http://www.coypu.org/ontologies/em-dat/Earthquake> <http://www.w3.org/2000/01/rdf-schema#label> "earthquake"@en .
<http://www.coypu.org/ontologies/em-dat/GeophysicalDisaster> <http://www.w3.org/2000/01/rdf-schema#label> "geophysical disaster"@en .
<http://www.coypu.org/ontologies/em-dat/EnergeticParticles> <http://www.w3.org/2000/01/rdf-schema#label> "energetic particles"@en .
<http://www.coypu.org/ontologies/em-dat/SpaceWeather> <http://www.w3.org/2000/01/rdf-schema#label> "space weather"@en .
<http://www.coypu.org/ontologies/em-dat/Explosion> <http://www.w3.org/2000/01/rdf-schema#label> "explosion"@en .
<http://www.coypu.org/ontologies/em-dat/ExtraTropicalStorm> <http://www.w3.org/2000/01/rdf-schema#label> "extra-tropical storm"@en .
<http://www.coypu.org/ontologies/em-dat/ExtraterrestrialDisaster> <http://www.w3.org/2000/01/rdf-schema#label> "extraterrestrial disaster"@en .
<http://www.coypu.org/ontologies/em-dat/MeteorologicalDisaster> <http://www.w3.org/2000/01/rdf-schema#label> "meteorological disaster"@en .
<http://www.coypu.org/ontologies/em-dat/Fire> <http://www.w3.org/2000/01/rdf-schema#label> "fire"@en .
<http://www.coypu.org/ontologies/em-dat/FlashFlood> <http://www.w3.org/2000/01/rdf-schema#label> "flash flood"@en .
<http://www.coypu.org/ontologies/em-dat/HydrologicalDisaster> <http://www.w3.org/2000/01/rdf-schema#label> "hydrological disaster"@en .
<http://www.coypu.org/ontologies/em-dat/Fog> <http://www.w3.org/2000/01/rdf-schema#label> "fog"@en .
<http://www.coypu.org/ontologies/em-dat/ForestFire> <http://www.w3.org/2000/01/rdf-schema#label> "forest fire"@en .
<http://www.coypu.org/ontologies/em-dat/Wildfire> <http://www.w3.org/2000/01/rdf-schema#label> "wildfire"@en .
<http://www.coypu.org/ontologies/em-dat/FrostOrFreeze> <http://www.w3.org/2000/01/rdf-schema#label> "frost/freeze"@en .
<http://www.coypu.org/ontologies/em-dat/SevereWinterConditions> <http://www.w3.org/2000/01/rdf-schema#label> "severe winter conditions"@en .
<http://www.coypu.org/ontologies/em-dat/FungalDisease> <http://www.w3.org/2000/01/rdf-schema#label> "fungal disease"@en .
<http://www.coypu.org/ontologies/em-dat/GasLeak> <http://www.w3.org/2000/01/rdf-schema#label> "gas leak"@en .
<http://www.coypu.org/ontologies/em-dat/GeomagneticStorm> <http://www.w3.org/2000/01/rdf-schema#label> "geomagnetic storm"@en .
<http://www.coypu.org/ontologies/em-dat/GlacialLakeOutburst> <http://www.w3.org/2000/01/rdf-schema#label> "glacial lake outburst"@en .
<http://www.coypu.org/ontologies/em-dat/Grasshopper> <http://www.w3.org/2000/01/rdf-schema#label> "grasshopper"@en .
<http://www.coypu.org/ontologies/em-dat/InsectInfestation> <http://www.w3.org/2000/01/rdf-schema#label> "insect infestation"@en .
<http://www.coypu.org/ontologies/em-dat/GroundMovement> <http://www.w3.org/2000/01/rdf-schema#label> "ground movement"@en .
<http://www.coypu.org/ontologies/em-dat/Hail> <http://www.w3.org/2000/01/rdf-schema#label> "hail"@en .
<http://www.coypu.org/ontologies/em-dat/HeatWave> <http://www.w3.org/2000/01/rdf-schema#label> "heat wave"@en .
<http://www.coypu.org/ontologies/em-dat/IceJamFlood> <http://www.w3.org/2000/01/rdf-schema#label> "ice jam flood"@en .
<http://www.coypu.org/ontologies/em-dat/TechnologicalDisaster> <http://www.w3.org/2000/01/rdf-schema#label> "technological disaster"@en .
<http://www.coypu.org/ontologies/em-dat/Lahar> <http://www.w3.org/2000/01/rdf-schema#label> "lahar"@en .
<http://www.coypu.org/ontologies/em-dat/LandFire> <http://www.w3.org/2000/01/rdf-schema#label> "land fire: brush, bush, pasture"@en .
<http://www.coypu.org/ontologies/em-dat/LavaFlow> <http://www.w3.org/2000/01/rdf-schema#label> "lava flow"@en .
<http://www.coypu.org/ontologies/em-dat/LightningOrThunderstorm> <http://www.w3.org/2000/01/rdf-schema#label> "lightning/thunderstorm"@en .
<http://www.coypu.org/ontologies/em-dat/Locust> <http://www.w3.org/2000/01/rdf-schema#label> "locust"@en .
<http://www.coypu.org/ontologies/em-dat/OilSpill> <http://www.w3.org/2000/01/rdf-schema#label> "oil spill"@en .
<http://www.coypu.org/ontologies/em-dat/Other> <http://www.w3.org/2000/01/rdf-schema#label> "other"@en .
<http://www.coypu.org/ontologies/em-dat/ParasiticDisease> <http://www.w3.org/2000/01/rdf-schema#label> "parasitic disease"@en .
<http://www.coypu.org/ontologies/em-dat/Poisoning> <http://www.w3.org/2000/01/rdf-schema#label> "poisoning"@en .
<http://www.coypu.org/ontologies/em-dat/PrionDisease> <http://www.w3.org/2000/01/rdf-schema#label> "prion disease"@en .
<http://www.coypu.org/ontologies/em-dat/PyroclasticFlow> <http://www.w3.org/2000/01/rdf-schema#label> "pyroclastic flow"@en .
<http://www.coypu.org/ontologies/em-dat/Radiation> <http://www.w3.org/2000/01/rdf-schema#label> "radiation"@en .
<http://www.coypu.org/ontologies/em-dat/Rail> <http://www.w3.org/2000/01/rdf-schema#label> "rail"@en .
<http://www.coypu.org/ontologies/em-dat/Rain> <http://www.w3.org/2000/01/rdf-schema#label> "rain"@en .
<http://www.coypu.org/ontologies/em-dat/RiverineFlood> <http://www.w3.org/2000/01/rdf-schema#label> "riverine flood"@en .
<http://www.coypu.org/ontologies/em-dat/Road> <http://www.w3.org/2000/01/rdf-schema#label> "road"@en .
<http://www.coypu.org/ontologies/em-dat/RockFall> <http://www.w3.org/2000/01/rdf-schema#label> "rock fall"@en .
<http://www.coypu.org/ontologies/em-dat/MassMovement_(dry)> <http://www.w3.org/2000/01/rdf-schema#label> "mass movement (dry)"@en .
<http://www.coypu.org/ontologies/em-dat/RogueWave> <http://www.w3.org/2000/01/rdf-schema#label> "rogue wave"@en .
<http://www.coypu.org/ontologies/em-dat/WaveAction> <http://www.w3.org/2000/01/rdf-schema#label> "wave action"@en .
<http://www.coypu.org/ontologies/em-dat/SandOrDustStorm> <http://www.w3.org/2000/01/rdf-schema#label> "sand/dust storm"@en .
<http://www.coypu.org/ontologies/em-dat/Seiche> <http://www.w3.org/2000/01/rdf-schema#label> "seiche"@en .
<http://www.coypu.org/ontologies/em-dat/SevereStorm> <http://www.w3.org/2000/01/rdf-schema#label> "severe storm"@en .
<http://www.coypu.org/ontologies/em-dat/Shockwave> <http://www.w3.org/2000/01/rdf-schema#label> "shockwave"@en .
<http://www.coypu.org/ontologies/em-dat/SnowOrIce> <http://www.w3.org/2000/01/rdf-schema#label> "snow/ice"@en .
<http://www.coypu.org/ontologies/em-dat/StormOrSurge> <http://www.w3.org/2000/01/rdf-schema#label> "storm/surge"@en .
<http://www.coypu.org/ontologies/em-dat/Tornado> <http://www.w3.org/2000/01/rdf-schema#label> "tornado"@en .
<http://www.coypu.org/ontologies/em-dat/TropicalStorm> <http://www.w3.org/2000/01/rdf-schema#label> "tropical storm"@en .
<http://www.coypu.org/ontologies/em-dat/Tsunami> <http://www.w3.org/2000/01/rdf-schema#label> "tsunami"@en .
<http://www.coypu.org/ontologies/em-dat/ViralDisease> <http://www.w3.org/2000/01/rdf-schema#label> "viral disease"@en .
<http://www.coypu.org/ontologies/em-dat/Water> <http://www.w3.org/2000/01/rdf-schema#label> "water"@en .
<http://www.coypu.org/ontologies/em-dat/Wind> <http://www.w3.org/2000/01/rdf-schema#label> "wind"@en .
<http://www.coypu.org/ontologies/em-dat/WinterStormOrBlizzard> <http://www.w3.org/2000/01/rdf-schema#label> "winter storm/blizzard"@en .
<http://www.coypu.org/ontologies/em-dat/Landslide(dry)> <http://www.w3.org/2000/01/rdf-schema#label> "landslide (dry)"@en .
<http://www.coypu.org/ontologies/em-dat/firstOrderAdminCode> <http://www.w3.org/2000/01/rdf-schema#label> "first order admin code"@en .
<http://www.coypu.org/ontologies/em-dat/> <http://www.w3.org/2000/01/rdf-schema#comment> "Crisis/hazard related taxonomy developed by CRED for disaster preparedness and humanitarian\nactions at national and international level"@en .
<http://www.coypu.org/ontologies/em-dat/TransportAccident> <http://www.w3.org/2000/01/rdf-schema#comment> "Disaster type term used in EM-DAT to describe technological transport accidents involving mechanised modes of transport. It comprises of four disaster subsets: accidents involving aeroplanes, helicopters, airships and balloons « Transport:Air »; accidents involving sailing boats, ferries, cruise ships, other boats « Transport:Boat »; accidents involving trains « Transport:Rail »; and accidents involving motor vehicles on roads and tracks « Transport:Road »."@en .
<http://www.coypu.org/ontologies/em-dat/Airburst> <http://www.w3.org/2000/01/rdf-schema#comment> "An explosion of a comet or meteoroid within the Earth’s atmosphere without striking the ground."@en .
<http://www.coypu.org/ontologies/em-dat/Impact> <http://www.w3.org/2000/01/rdf-schema#comment> "A type of extraterrestrial hazard caused by the collision of the Earth with a meteoroid, asteroid or comet."@en .
<http://www.coypu.org/ontologies/em-dat/AnimalAccident> <http://www.w3.org/2000/01/rdf-schema#comment> "Human encounters with dangerous or exotic animals in both urban and rural developments."@en .
<http://www.coypu.org/ontologies/em-dat/BiologicalDisaster> <http://www.w3.org/2000/01/rdf-schema#comment> "A hazard caused by the exposure to living organisms and their toxic substances (e.g. venom, mold) or vector-borne diseases that they may carry. Examples are venomous wildlife and insects, poisonous plants, and mosquitoes carrying disease-causing agents such as parasites, bacteria, or viruses (e.g. malaria)."@en .
<http://www.coypu.org/ontologies/em-dat/AshFall> <http://www.w3.org/2000/01/rdf-schema#comment> "Fine (less than 4 mm in diameter) unconsolidated volcanic debris blown into the atmosphere during an eruption; can remain airborne for long periods of time and travel considerable distance from the source."@en .
<http://www.coypu.org/ontologies/em-dat/VolcanicActivity> <http://www.w3.org/2000/01/rdf-schema#comment> "A type of volcanic event near an opening/vent in the Earth’s surface including volcanic eruptions of lava, ash, hot vapour, gas, and pyroclastic material."@en .
<http://www.coypu.org/ontologies/em-dat/Avalanche> <http://www.w3.org/2000/01/rdf-schema#comment> "A large mass of loosened earth material, snow, or ice that slides, flows or falls rapidly down a mountainside under the force of gravity.\n\n- Snow Avalanche: Rapid downslope movement of a mix of snow and ice.\n- Debris Avalanche: The sudden and very rapid downslope movement of unsorted mass of rock and soil. There are two general types of debris avalanches - a cold debris avalanche usually results from an unstable slope suddenly collapsing whereas a hot debris avalanche results from volcanic activity leading to slope instability and collapse."@en .
<http://www.coypu.org/ontologies/em-dat/Landslide(wet)> <http://www.w3.org/2000/01/rdf-schema#comment> "Any kind of moderate to rapid soil movement incl. lahar, mudslide, debris flow. A landslide is the movement of soil or rock controlled by gravity and the speed of the movement usually ranges between slow and rapid, but not very slow. It can be superficial or deep, but the materials have to make up a mass that is a portion of the slope or the slope itself. The movement has to be downward and outward with a free face."@en .
<http://www.coypu.org/ontologies/em-dat/Bacterial_Disease> <http://www.w3.org/2000/01/rdf-schema#comment> "An unusual increase in the number of incidents caused by the exposure to bacteria either through skin contact, ingestion or inhalation. Examples include salmonella, MSRA, and cholera, among others."@en .
<http://www.coypu.org/ontologies/em-dat/Epidemic> <http://www.w3.org/2000/01/rdf-schema#comment> "Either an unusual increase in the number of cases of an infectious disease, which already exists in the region or population concerned; or the appearance of an infection previously absent from a region."@en .
<http://www.coypu.org/ontologies/em-dat/ChemicalSpill> <http://www.w3.org/2000/01/rdf-schema#comment> "Accident release occurring during the production, transportation or handling of hazardous chemical substances."@en .
<http://www.coypu.org/ontologies/em-dat/IndustrialAccident> <http://www.w3.org/2000/01/rdf-schema#comment> "Disaster type term used in EM-DAT to describe technological accidents of an industrial nature/involving industrial buildings (e.g. factories)."@en .
<http://www.coypu.org/ontologies/em-dat/ClimatologicalDisaster> <http://www.w3.org/2000/01/rdf-schema#comment> "A hazard caused by long-lived, meso- to macro-scale atmospheric processes ranging from intra-seasonal to multi-decadal climate variability."@en .
<http://www.coypu.org/ontologies/em-dat/CoastalFlood> <http://www.w3.org/2000/01/rdf-schema#comment> "Higher-than-normal water levels along the coast caused by tidal changes or thunderstorms that result in ﬂooding, which can last from days to weeks."@en .
<http://www.coypu.org/ontologies/em-dat/Flood> <http://www.w3.org/2000/01/rdf-schema#comment> "A general term for the overﬂow of water from a stream channel onto normally dry land in the ﬂoodplain (riverine ﬂooding), higher-than- normal levels along the coast and in lakes or reservoirs (coastal ﬂooding) as well as ponding of water at or near the point where the rain fell (ﬂash ﬂoods)."@en .
<http://www.coypu.org/ontologies/em-dat/ColdWave> <http://www.w3.org/2000/01/rdf-schema#comment> "A period of abnormally cold weather. Typically a cold wave lasts two or more days and may be aggravated by high winds. The exact temperature criteria for what constitutes a cold wave vary by location."@en .
<http://www.coypu.org/ontologies/em-dat/Collapse> <http://www.w3.org/2000/01/rdf-schema#comment> "Accident involving the collapse of building or structure. Can either involve industrial structures or domestic / non-industrial structures."@en .
<http://www.coypu.org/ontologies/em-dat/MiscelleanousAccident> <http://www.w3.org/2000/01/rdf-schema#comment> "Disaster type term used in EM-DAT to describe technological accidents of a non-industrial or transport nature (e.g. houses)."@en .
<http://www.coypu.org/ontologies/em-dat/ConvectiveStorm> <http://www.w3.org/2000/01/rdf-schema#comment> "A type of meteorological hazard generated by the heating of air and the availability of moist and unstable air masses. Convective storms range from localised thunderstorms (with heavy rain and/or hail, lightning, high winds, tornadoes) to meso-scale, multi-day events."@en .
<http://www.coypu.org/ontologies/em-dat/Disaster> <http://www.w3.org/2000/01/rdf-schema#comment> "Situation or event, which overwhelms local capacity, necessitating a request to national or international level for external assistance (definition considered in EM-DAT); An unforeseen and often sudden event that causes great damage, destruction and human suffering. Though often caused by nature, disasters can have human origins."@en .
<http://www.coypu.org/ontologies/em-dat/Drought> <http://www.w3.org/2000/01/rdf-schema#comment> "An extended period of unusually low precipitation that produces a shortage of water for people, animals and plants. Drought is diﬀerent from most other hazards in that it develops slowly, sometimes even over years, and its onset is generally diﬃcult to detect. Drought is not solely a physical phenomenon because its impacts can be exacerbated by human activities and water supply demands. Drought is therefore often deﬁned both conceptually and operationally. Operational deﬁnitions of drought, meaning the degree of precipitation reduction that constitutes a drought, vary by locality, climate and environmental sector."@en .
<http://www.coypu.org/ontologies/em-dat/Earthquake> <http://www.w3.org/2000/01/rdf-schema#comment> "Sudden movement of a block of the Earth’s crust along a geological fault and associated ground shaking."@en .
<http://www.coypu.org/ontologies/em-dat/GeophysicalDisaster> <http://www.w3.org/2000/01/rdf-schema#comment> "A hazard originating from solid earth. This term is used interchangeably with the term geological hazard."@en .
<http://www.coypu.org/ontologies/em-dat/EnergeticParticles> <http://www.w3.org/2000/01/rdf-schema#comment> "Emissions from solar radiation storms consisting of pieces of matter (e.g., protons and other charged particles) moving at very high speed. The magnetosphere and atmosphere block (solar) energetic particles (SEP) from reaching humans on Earth but they are damaging to the electronics of space-borne technology (such as satellites) and pose a radiation hazard to life in space and aircrafts travelling at high altitudes."@en .
<http://www.coypu.org/ontologies/em-dat/Explosion> <http://www.w3.org/2000/01/rdf-schema#comment> "Explosions involving buildings or structures. Can either involve industrial structures or domestic / non-industrial structures."@en .
<http://www.coypu.org/ontologies/em-dat/ExtraTropicalStorm> <http://www.w3.org/2000/01/rdf-schema#comment> "A type of low-pressure cyclonic system in the middle and high latitudes (also called mid-latitude cyclone) that primarily gets its energy from the horizontal temperature contrasts (fronts) in the atmosphere. When associated with cold fronts, extratropical cyclones may be particularly damaging (e.g. European winter/windstorm, Nor’easter)."@en .
<http://www.coypu.org/ontologies/em-dat/ExtraterrestrialDisaster> <http://www.w3.org/2000/01/rdf-schema#comment> "A hazard caused by asteroids, meteoroids, and comets as they pass near-earth, enter the Earth’s atmosphere, and/or strike the Earth, and by changes in interplanetary conditions that effect the Earth’s magnetosphere, ionosphere, and thermosphere."@en .
<http://www.coypu.org/ontologies/em-dat/MeteorologicalDisaster> <http://www.w3.org/2000/01/rdf-schema#comment> "A hazard caused by short-lived, micro- to meso-scale extreme weather and atmospheric conditions that last from minutes to days."@en .
<http://www.coypu.org/ontologies/em-dat/Fire> <http://www.w3.org/2000/01/rdf-schema#comment> "Urban fire involving buildings or structures. Can either involve industrial structures or domestic / non-industrial structures."@en .
<http://www.coypu.org/ontologies/em-dat/FlashFlood> <http://www.w3.org/2000/01/rdf-schema#comment> "Rapid inland floods due to intense rainfall A flash flood describes sudden flooding with short duration. In sloped terrain the water flows rapidly with a high destruction potential. In flat terrain the rainwater cannot infiltrate into the ground or run off (due to small slope) as quickly as it falls. Flash floods typically are associated with thunderstorms. A flash flood can occur at virtually any place."@en .
<http://www.coypu.org/ontologies/em-dat/HydrologicalDisaster> <http://www.w3.org/2000/01/rdf-schema#comment> "A hazard caused by the occurrence, movement, and distribution of surface and subsurface freshwater and saltwater."@en .
<http://www.coypu.org/ontologies/em-dat/Fog> <http://www.w3.org/2000/01/rdf-schema#comment> "Water droplets that are suspended in the air near the Earth’s surface. Fog is simply a cloud that is in contact with the ground."@en .
<http://www.coypu.org/ontologies/em-dat/ForestFire> <http://www.w3.org/2000/01/rdf-schema#comment> "A type of wildﬁre in a wooded area."@en .
<http://www.coypu.org/ontologies/em-dat/Wildfire> <http://www.w3.org/2000/01/rdf-schema#comment> "Any uncontrolled and non-prescribed combustion or burning of plants in a natural setting such as a forest, grassland, brush land or tundra, which consumes the natural fuels and spreads based on environmental conditions (e.g., wind, topography). Wildﬁres can be triggered by lightning or human actions."@en .
<http://www.coypu.org/ontologies/em-dat/SevereWinterConditions> <http://www.w3.org/2000/01/rdf-schema#comment> "Damage caused by snow and ice. Winter damage refers to damage to buildings, infrastructure, traffic (esp. navigation) inflicted by snow and ice in form of snow pressure, freezing rain, frozen waterways etc."@en .
<http://www.coypu.org/ontologies/em-dat/FungalDisease> <http://www.w3.org/2000/01/rdf-schema#comment> "Exposure to fungi either through skin contact, ingestion or inhalation of spores resulting in an unusual increase in the number of incidents. Examples are fungal pneumonia, fungal meningitis, etc."@en .
<http://www.coypu.org/ontologies/em-dat/GeomagneticStorm> <http://www.w3.org/2000/01/rdf-schema#comment> "A type of extraterrestrial hazard caused by solar wind shockwaves that temporarily disturb the Earth’s magnetosphere. Geomagnetic storms can disrupt power grids, spacecraft operations, and satellite communications."@en .
<http://www.coypu.org/ontologies/em-dat/GlacialLakeOutburst> <http://www.w3.org/2000/01/rdf-schema#comment> "A ﬂood that occurs when water dammed by a glacier or moraine is suddenly released. Glacial lakes can be at the front of the glacier (marginal lake) or below the ice sheet (sub-glacial lake)."@en .
<http://www.coypu.org/ontologies/em-dat/InsectInfestation> <http://www.w3.org/2000/01/rdf-schema#comment> "Pervasive influx and development of insects or parasites affecting humans, animals, crops and materials."@en .
<http://www.coypu.org/ontologies/em-dat/GroundMovement> <http://www.w3.org/2000/01/rdf-schema#comment> "Surface displacement of earthen materials due to ground shaking triggered by earthquakes or volcanic eruptions."@en .
<http://www.coypu.org/ontologies/em-dat/Hail> <http://www.w3.org/2000/01/rdf-schema#comment> "Storm with hailstones as dominant type of precipitation. A hail storm is a type of storm that is characterised by hail as the dominant part of its precipitation. The size of the hailstones can vary between pea size (6mm) and softball size (112mm) and therefore cause considerable damage."@en .
<http://www.coypu.org/ontologies/em-dat/IceJamFlood> <http://www.w3.org/2000/01/rdf-schema#comment> "The accumulation of ﬂoating ice restricting or blocking a river’s ﬂow and drainage. Ice jams tend to develop near river bends and obstructions (e.g. bridges)."@en .
<http://www.coypu.org/ontologies/em-dat/Lahar> <http://www.w3.org/2000/01/rdf-schema#comment> "Hot or cold mixture of earthen material ﬂowing on the slope of a volcano either during or between volcanic eruptions"@en .
<http://www.coypu.org/ontologies/em-dat/LavaFlow> <http://www.w3.org/2000/01/rdf-schema#comment> "The ejected magma that moves as a liquid mass downslope from a volcano during an eruption."@en .
<http://www.coypu.org/ontologies/em-dat/LightningOrThunderstorm> <http://www.w3.org/2000/01/rdf-schema#comment> "Hazards/losses caused by lightning stroke. Lightning is an atmospheric discharge of electricity, which typically occurs during thunderstorms, and sometimes during volcanic eruptions or dust storms."@en .
<http://www.coypu.org/ontologies/em-dat/ParasiticDisease> <http://www.w3.org/2000/01/rdf-schema#comment> "Exposure to a parasite–an organism living on or in a host–causes an unusual increase in the number of incidents. Exposure to parasites occurs mostly through contaminated water, food or contact with insects, animals (zoonotic), pets, etc. Examples are malaria, chagas disease, giardiasis and trichinellosis."@en .
<http://www.coypu.org/ontologies/em-dat/Poisoning> <http://www.w3.org/2000/01/rdf-schema#comment> "Poisoning of atmosphere or water courses due to industrial sources."@en .
<http://www.coypu.org/ontologies/em-dat/PrionDisease> <http://www.w3.org/2000/01/rdf-schema#comment> "A type of biological hazard caused by prion proteins. Prion diseases or transmissible spongiform encephalopathies (TSEs) are a family of rare progressive neurodegenerative disorders that aﬀect both humans and animals characterised by long incubation periods and neural loss. Examples are Bovine Spongiform Encephalophathy (BSE), Creutzfeldt- Jakob-Disease (CJD), Kuru, etc."@en .
<http://www.coypu.org/ontologies/em-dat/PyroclasticFlow> <http://www.w3.org/2000/01/rdf-schema#comment> "Extremely hot gases, ash, and other materials of more than 1,000 degrees Celsius that rapidly ﬂow down the ﬂank of a volcano (more than 700 km/h) during an eruption."@en .
<http://www.coypu.org/ontologies/em-dat/Rain> <http://www.w3.org/2000/01/rdf-schema#comment> "Water vapour condenses in the atmosphere to form water droplets that fall to the Earth."@en .
<http://www.coypu.org/ontologies/em-dat/MassMovement_(dry)> <http://www.w3.org/2000/01/rdf-schema#comment> "Any type of downslope movement of earth materials."@en .
<http://www.coypu.org/ontologies/em-dat/RogueWave> <http://www.w3.org/2000/01/rdf-schema#comment> "An unusual single crest of an ocean wave far out at sea that is much higher and/or steeper than other waves in the prevailing swell system"@en .
<http://www.coypu.org/ontologies/em-dat/SandOrDustStorm> <http://www.w3.org/2000/01/rdf-schema#comment> "A sandstorm/dust storm typically occurs in arid or semi-arid regions if high wind speeds cause the transportation of small particles like sand or fine clastic sediment by saltation and/or suspension. e.g. in deserts."@en .
<http://www.coypu.org/ontologies/em-dat/Seiche> <http://www.w3.org/2000/01/rdf-schema#comment> "A standing wave of water in a large semi- or fully-enclosed body of water (lakes or bays) created by strong winds and/or a large barometric pressure gradient."@en .
<http://www.coypu.org/ontologies/em-dat/Shockwave> <http://www.w3.org/2000/01/rdf-schema#comment> "A shockwave carries energy from a disturbance through a medium (solid, liquid, gas) similar to a wave though it travels at much higher speed. It can be a type of extraterrestrial hazard caused by the explosion (airburst) or impact of meteorites that generate energy shockwaves capable of shattering glass, collapsing walls, etc."@en .
<http://www.coypu.org/ontologies/em-dat/StormOrSurge> <http://www.w3.org/2000/01/rdf-schema#comment> "An abnormal rise in sea level generated by a tropical cyclone or other intense storms."@en .
<http://www.coypu.org/ontologies/em-dat/Tornado> <http://www.w3.org/2000/01/rdf-schema#comment> "A violently rotating column of air that reaches the ground or open water (waterspout)."@en .
<http://www.coypu.org/ontologies/em-dat/TropicalStorm> <http://www.w3.org/2000/01/rdf-schema#comment> "A tropical storm originates over tropical or subtropical waters. It is characterised by a warm-core, non-frontal synoptic-scale cyclone with a low pressure centre, spiral rain bands and strong winds. Depending on their location, tropical cyclones are referred to as hurricanes (Atlantic, Northeast Paciﬁc), typhoons (Northwest Paciﬁc), or cyclones (South Paciﬁc and Indian Ocean)."@en .
<http://www.coypu.org/ontologies/em-dat/Tsunami> <http://www.w3.org/2000/01/rdf-schema#comment> "« wave in the port » in Japanese: A series of waves (with long wavelengths when traveling across the deep ocean) that are generated by a displacement of massive amounts of water through underwater earthquakes, volcanic eruptions or landslides. Tsunami waves travel at very high speed across the ocean but as they begin to reach shallow water they slow down and the wave grows steeper."@en .
<http://www.coypu.org/ontologies/em-dat/Wind> <http://www.w3.org/2000/01/rdf-schema#comment> "Diﬀerences in air pressure resulting in the horizontal motion of air. The greater the diﬀerence in pressure, the stronger the wind. Wind moves from high pressure toward low pressure."@en .
<http://www.coypu.org/ontologies/em-dat/WinterStormOrBlizzard> <http://www.w3.org/2000/01/rdf-schema#comment> "A low pressure system in winter months with signiﬁcant accumulations of snow, freezing rain, sleet or ice. A blizzard is a severe snow storm with winds exceeding 35 mph (56 km/h) for three or more hours, producing reduced visibility (less than 0.25 mile (400 m))."@en .
<http://www.coypu.org/ontologies/em-dat/Landslide(dry)> <http://www.w3.org/2000/01/rdf-schema#comment> "Any kind of moderate to rapid soil movement incl. lahar, mudslide, debris flow. A landslide is the movement of soil or rock controlled by gravity and the speed of the movement usually ranges between slow and rapid, but not very slow. It can be superficial or deep, but the materials have to make up a mass that is a portion of the slope or the slope itself. The movement has to be downward and outward with a free face."@en .
_:node807 <http://www.w3.org/1999/02/22-rdf-syntax-ns#first> <http://www.coypu.org/ontologies/em-dat/IndustrialAccident> .
_:node808 <http://www.w3.org/1999/02/22-rdf-syntax-ns#first> <http://www.coypu.org/ontologies/em-dat/MiscelleanousAccident> .
_:node810 <http://www.w3.org/1999/02/22-rdf-syntax-ns#first> <http://www.coypu.org/ontologies/em-dat/IndustrialAccident> .
_:node811 <http://www.w3.org/1999/02/22-rdf-syntax-ns#first> <http://www.coypu.org/ontologies/em-dat/MiscelleanousAccident> .
_:node813 <http://www.w3.org/1999/02/22-rdf-syntax-ns#first> <http://www.coypu.org/ontologies/em-dat/IndustrialAccident> .
_:node814 <http://www.w3.org/1999/02/22-rdf-syntax-ns#first> <http://www.coypu.org/ontologies/em-dat/MiscelleanousAccident> .
_:node816 <http://www.w3.org/1999/02/22-rdf-syntax-ns#first> <http://www.coypu.org/ontologies/em-dat/IndustrialAccident> .
_:node817 <http://www.w3.org/1999/02/22-rdf-syntax-ns#first> <http://www.coypu.org/ontologies/em-dat/MiscelleanousAccident> .
_:node807 <http://www.w3.org/1999/02/22-rdf-syntax-ns#rest> _:node808 .
_:node808 <http://www.w3.org/1999/02/22-rdf-syntax-ns#rest> <http://www.w3.org/1999/02/22-rdf-syntax-ns#nil> .
_:node810 <http://www.w3.org/1999/02/22-rdf-syntax-ns#rest> _:node811 .
_:node811 <http://www.w3.org/1999/02/22-rdf-syntax-ns#rest> <http://www.w3.org/1999/02/22-rdf-syntax-ns#nil> .
_:node813 <http://www.w3.org/1999/02/22-rdf-syntax-ns#rest> _:node814 .
_:node814 <http://www.w3.org/1999/02/22-rdf-syntax-ns#rest> <http://www.w3.org/1999/02/22-rdf-syntax-ns#nil> .
_:node816 <http://www.w3.org/1999/02/22-rdf-syntax-ns#rest> _:node817 .
_:node817 <http://www.w3.org/1999/02/22-rdf-syntax-ns#rest> <http://www.w3.org/1999/02/22-rdf-syntax-ns#nil> .
<http://www.coypu.org/ontologies/em-dat/> <http://www.w3.org/2002/07/owl#versionIRI> <http://www.coypu.org/ontologies/em-dat/0.1.0> .
_:node806 <http://www.w3.org/2002/07/owl#unionOf> _:node807 .
_:node809 <http://www.w3.org/2002/07/owl#unionOf> _:node810 .
_:node812 <http://www.w3.org/2002/07/owl#unionOf> _:node813 .
_:node815 <http://www.w3.org/2002/07/owl#unionOf> _:node816 .
<http://www.coypu.org/ontologies/em-dat/> <http://purl.org/dc/terms/preferedNamespaceUri> "http://www.coypu.org/ontologies/em-dat/" .
<http://www.coypu.org/ontologies/em-dat/> <http://purl.org/dc/terms/preferredNamespacePrefix> "emdat" .
<http://www.coypu.org/ontologies/em-dat/> <http://www.coypu.org/ontologies/em-dat/> "" .
<http://www.coypu.org/ontologies/em-dat/> <http://www.coypu.org/ontologies/em-dat/firstOrderAdminCode> "String" .
