@prefix : <https://schema.coypu.org/gta/> .
@prefix coy: <https://schema.coypu.org/gta/> .
@prefix owl: <http://www.w3.org/2002/07/owl#> .
@prefix rdf: <http://www.w3.org/1999/02/22-rdf-syntax-ns#> .
@prefix xml: <http://www.w3.org/XML/1998/namespace> .
@prefix xsd: <http://www.w3.org/2001/XMLSchema#> .
@prefix rdfs: <http://www.w3.org/2000/01/rdf-schema#> .
@base <https://schema.coypu.org/gta/> .

<https://schema.coypu.org/gta/> rdf:type owl:Ontology ;
                                 owl:versionIRI <https://schema.coypu.org/gta/0.1.0> ;
                                 rdfs:comment "An ontology for modeling global trade alerts mainly inspired by Global Trade Alerts repository."@en ;
                                 rdfs:label "Global Trade Alerts Ontology"@en ;
                                 rdfs:seeAlso "https://www.globaltradealert.org/" ;
                                 owl:versionInfo "v0.1.0" .

#################################################################
#    Object Properties
#################################################################

###  https://schema.coypu.org/gta/hasAffectedJurisdiction
coy:hasAffectedJurisdiction rdf:type owl:ObjectProperty ;
                            rdfs:domain coy:Intervention ;
                            rdfs:range coy:Jurisdiction .


###  https://schema.coypu.org/gta/hasAffectedProduct
coy:hasAffectedProduct rdf:type owl:ObjectProperty ;
                       rdfs:domain coy:Intervention .


###  https://schema.coypu.org/gta/hasAffectedSector
coy:hasAffectedSector rdf:type owl:ObjectProperty ;
                      rdfs:domain coy:Intervention ;
                      rdfs:range coy:Sector .


###  https://schema.coypu.org/gta/hasGTAEvaluation
coy:hasGTAEvaluation rdf:type owl:ObjectProperty ;
                     rdfs:domain coy:Intervention ;
                     rdfs:range coy:GTAEvaluation ;
                     rdfs:label "has GTA evaluation"@en .


###  https://schema.coypu.org/gta/hasImplementingJurisdiction
coy:hasImplementingJurisdiction rdf:type owl:ObjectProperty ;
                                rdfs:range coy:Jurisdiction .


###  https://schema.coypu.org/gta/hasIntervention
coy:hasIntervention rdf:type owl:ObjectProperty ;
                    rdfs:domain coy:StateAct ;
                    rdfs:range coy:Intervention ;
                    rdfs:label "has intervention"@en .


###  https://schema.coypu.org/gta/hasInterventionType
coy:hasInterventionType rdf:type owl:ObjectProperty ;
                        rdfs:domain coy:Intervention ;
                        rdfs:range coy:InterventionType .


#################################################################
#    Data properties
#################################################################

###  https://schema.coypu.org/gta/hasAnnouncementDate
coy:hasAnnouncementDate rdf:type owl:DatatypeProperty ;
                        rdfs:comment "The issuance date of the documented government statement."@en ;
                        rdfs:label "Announcement date"@en .


###  https://schema.coypu.org/gta/hasImplementationDate
coy:hasImplementationDate rdf:type owl:DatatypeProperty ;
                          rdfs:comment "The date the documented change is enforced."@en ;
                          rdfs:label "Implementation date"@en .


###  https://schema.coypu.org/gta/hasInterventionID
coy:hasInterventionID rdf:type owl:DatatypeProperty ,
                               owl:FunctionalProperty ;
                      rdfs:domain coy:Intervention ;
                      rdfs:label "has intervention ID"@en .


###  https://schema.coypu.org/gta/hasInvestigationStatusDate
coy:hasInvestigationStatusDate rdf:type owl:DatatypeProperty ;
                               rdfs:label "Investigation status date"@en .


###  https://schema.coypu.org/gta/hasProductID
coy:hasProductID rdf:type owl:DatatypeProperty ;
                 rdfs:range [ rdf:type rdfs:Datatype ;
                              owl:onDatatype xsd:string ;
                              owl:withRestrictions ( [ xsd:pattern "[0-9]{6}"
                                                     ]
                                                   )
                            ] ;
                 rdfs:comment """The GTA uses the Harmonised System (HS, version 2012) at the 6-digit level. At this level, the Harmonised
System includes more than 5’000 different products. Each product is commonly referred to as its own “tariff
line”. The details of this classification and its correspondence to others are available from the World Customs
Organisation. The United Nations Statistics Division published a helpful summary."""@en ;
                 rdfs:label "has product ID"@en .


###  https://schema.coypu.org/gta/hasProlongationAnnouncementDate
coy:hasProlongationAnnouncementDate rdf:type owl:DatatypeProperty ;
                                    rdfs:comment """The date on which the prolongation of a temporary change was
communicated."""@en ;
                                    rdfs:label "Prolongation announcement date"@en .


###  https://schema.coypu.org/gta/hasProlongationImplementationDate
coy:hasProlongationImplementationDate rdf:type owl:DatatypeProperty ;
                                      rdfs:comment """The date the prolongation became effective i.e. the day after the
previously sought removal date."""@en ;
                                      rdfs:label "Prolongation implementation date"@en .


###  https://schema.coypu.org/gta/hasProlongationRemovalDate
coy:hasProlongationRemovalDate rdf:type owl:DatatypeProperty ;
                               rdfs:comment """The date the prolongation ends i.e. the new removal date as implied by
this prolongation."""@en ;
                               rdfs:label "Prolongation removal date"@en .


###  https://schema.coypu.org/gta/hasRemovalDate
coy:hasRemovalDate rdf:type owl:DatatypeProperty ;
                   rdfs:comment """The date the documented change is either withdrawn or fully replaced by a further
change. Note that changes that have only been partially replaced or withdrawn do not include a
removal date."""@en ;
                   rdfs:label "Removal date"@en .


###  https://schema.coypu.org/gta/hasSectorID
coy:hasSectorID rdf:type owl:DatatypeProperty ,
                         owl:FunctionalProperty ;
                rdfs:domain coy:Sector ;
                rdfs:range [ rdf:type rdfs:Datatype ;
                             owl:onDatatype xsd:string ;
                             owl:withRestrictions ( [ xsd:pattern "[0-9]{3}"
                                                    ]
                                                  )
                           ] ;
                rdfs:comment """The GTA uses the Common Product Classification (CPC, version 2.1) at the 3-digit level. The details of this
classification and its correspondence to others are available from the United Nations Statistics Division."""@en ;
                rdfs:label "has sector ID"@en .


###  https://schema.coypu.org/gta/hasStateActID
coy:hasStateActID rdf:type owl:DatatypeProperty ,
                           owl:FunctionalProperty ;
                  rdfs:domain coy:StateAct ;
                  rdfs:label "has state act ID"@en .


###  https://schema.coypu.org/gta/hasStateActTitle
coy:hasStateActTitle rdf:type owl:DatatypeProperty ;
                     rdfs:range xsd:string ;
                     rdfs:label "has state act title"@en .


###  https://schema.coypu.org/gta/hasTerminationAnnouncementDate
coy:hasTerminationAnnouncementDate rdf:type owl:DatatypeProperty ;
                                   rdfs:subPropertyOf owl:topDataProperty ;
                                   rdfs:comment """The date on which the premature termination of a temporary
change was communicated."""@en ;
                                   rdfs:label "Termination announcement date"@en .


###  https://schema.coypu.org/gta/hasTerminationImplementationDate
coy:hasTerminationImplementationDate rdf:type owl:DatatypeProperty ;
                                     rdfs:comment """The date the premature termination became effective i.e. the day
after the previously sought removal date."""@en ;
                                     rdfs:label "Termination implementation date"@en .


#################################################################
#    Classes
#################################################################

###  https://schema.coypu.org/gta/AffectedCommercialFlow
coy:AffectedCommercialFlow rdf:type owl:Class ;
                           rdfs:comment """The affected commercial flow field includes the predominantly affected flow direction. There are three
potential values. Only one value can be assigned to each intervention."""@en ;
                           rdfs:label "Affected commercial flow"@en .


###  https://schema.coypu.org/gta/CapitalControlsAndExchangeRatePolicy
coy:CapitalControlsAndExchangeRatePolicy rdf:type owl:Class ;
                                         rdfs:subClassOf coy:InterventionType ;
                                         rdfs:label "Capital controls and exchange rate policy"@en .


###  https://schema.coypu.org/gta/ExportAndImportPolicyInstruments
coy:ExportAndImportPolicyInstruments rdf:type owl:Class ;
                                     rdfs:subClassOf coy:InterventionType ;
                                     rdfs:label "Export and import policy instruments"@en .


###  https://schema.coypu.org/gta/ForeignInvestmentPolicy
coy:ForeignInvestmentPolicy rdf:type owl:Class ;
                            rdfs:subClassOf coy:InterventionType ;
                            rdfs:label "Foreign investment policy"@en .


###  https://schema.coypu.org/gta/GTAEvaluation
coy:GTAEvaluation rdf:type owl:Class ;
                  owl:equivalentClass [ rdf:type owl:Class ;
                                        owl:oneOf ( coy:AmberTriangle
                                                    coy:GreenTriangle
                                                    coy:RedTriangle
                                                  )
                                      ] ;
                  rdfs:comment "The direction of the change for each intervention. The evaluation is signalled by a triangle in one of three different colours."@en ;
                  rdfs:label "GTA evaluation"@en .


###  https://schema.coypu.org/gta/ImplementationLevel
coy:ImplementationLevel rdf:type owl:Class ;
                        rdfs:comment """The GTA database differentiates the announcements of different government levels or agencies. In total, it
distinguishes 6 different actors."""@en ;
                        rdfs:label "Implementation level"@en .


###  https://schema.coypu.org/gta/Intervention
coy:Intervention rdf:type owl:Class ;
                 rdfs:comment "Each state act in the GTA database consists of one or more interventions. The interventions represent the used policy instrument plus the direction of the induced change (liberalising or harmful). The clear majority of GTA database entries are state acts with a single associated intervention. For example, the announcement of a new production subsidy to steel producers would be recorded as one state act with one intervention."@en ;
                 rdfs:label "intervention"@en .


###  https://schema.coypu.org/gta/InterventionType
coy:InterventionType rdf:type owl:Class ;
                     rdfs:subClassOf owl:Thing ;
                     rdfs:label "intervention type"@en .


###  https://schema.coypu.org/gta/Jurisdiction
coy:Jurisdiction rdf:type owl:Class ;
                 rdfs:label "jurisdiction"@en .


###  https://schema.coypu.org/gta/LaborForceMigrationPolicy
coy:LaborForceMigrationPolicy rdf:type owl:Class ;
                              rdfs:subClassOf coy:InterventionType ;
                              rdfs:label "Labor force migration policy"@en .


###  https://schema.coypu.org/gta/LocalisationPolicy
coy:LocalisationPolicy rdf:type owl:Class ;
                       rdfs:subClassOf coy:InterventionType ;
                       rdfs:label "Localisation policy"@en .


###  https://schema.coypu.org/gta/OtherInstruments
coy:OtherInstruments rdf:type owl:Class ;
                     rdfs:subClassOf coy:InterventionType ;
                     rdfs:label "Other instruments"@en .


###  https://schema.coypu.org/gta/PublicProcurementPolicy
coy:PublicProcurementPolicy rdf:type owl:Class ;
                            rdfs:subClassOf coy:InterventionType ;
                            rdfs:label "Public procurement policy"@en .


###  https://schema.coypu.org/gta/Sector
coy:Sector rdf:type owl:Class ;
           rdfs:label "sector"@en .


###  https://schema.coypu.org/gta/StateAct
coy:StateAct rdf:type owl:Class ;
             rdfs:comment """For the GTA database, a state act is equivalent to an announcement by a government body. Each announcement documented by the GTA team includes at least one new and credible promise for change in market conditions at home or abroad.
Each state act in the GTA database consists of one or more interventions. The interventions represent the used policy instrument plus the direction of the induced change (liberalising or harmful). The clear majority of GTA database entries are state acts with a single associated intervention. For example, the announcement of a new production subsidy to steel producers would be recorded as one state act with one intervention."""@en ;
             rdfs:label "state act"@en .


###  https://schema.coypu.org/gta/SubsidiesAndStateAid
coy:SubsidiesAndStateAid rdf:type owl:Class ;
                         rdfs:subClassOf coy:InterventionType ;
                         rdfs:label "Subsidies and state aid"@en .


###  https://schema.coypu.org/gta/TradeDefenceInstruments
coy:TradeDefenceInstruments rdf:type owl:Class ;
                            rdfs:subClassOf coy:InterventionType ;
                            rdfs:label "Trade defence instruments"@en .


#################################################################
#    Individuals
#################################################################

###  https://schema.coypu.org/gta/AmberTriangle
coy:AmberTriangle rdf:type owl:NamedIndividual ,
                           coy:GTAEvaluation ;
                  rdfs:comment "The intervention likely involves discrimination against foreign commercial interests."@en ;
                  rdfs:label "amber triangle"@en .


###  https://schema.coypu.org/gta/Anti-Circumvention
coy:Anti-Circumvention rdf:type owl:NamedIndividual ,
                                coy:TradeDefenceInstruments ;
                       rdfs:label "Anti-Circumvention"@en .


###  https://schema.coypu.org/gta/Anti-Dumping
coy:Anti-Dumping rdf:type owl:NamedIndividual ,
                          coy:TradeDefenceInstruments ;
                 rdfs:label "Anti-Dumping"@en .


###  https://schema.coypu.org/gta/Anti-Subsidy
coy:Anti-Subsidy rdf:type owl:NamedIndividual ,
                          coy:TradeDefenceInstruments ;
                 rdfs:label "Anti-Subsidy"@en .


###  https://schema.coypu.org/gta/CompetitiveDevaluation
coy:CompetitiveDevaluation rdf:type owl:NamedIndividual ,
                                    coy:CapitalControlsAndExchangeRatePolicy ;
                           rdfs:label "Competitive devaluation"@en .


###  https://schema.coypu.org/gta/ControlOnPersonalTransactions
coy:ControlOnPersonalTransactions rdf:type owl:NamedIndividual ,
                                           coy:CapitalControlsAndExchangeRatePolicy ;
                                  rdfs:label "Control on personal transactions"@en .


###  https://schema.coypu.org/gta/ControlsOnCommercialTransactionsAndInvestmentInstruments
coy:ControlsOnCommercialTransactionsAndInvestmentInstruments rdf:type owl:NamedIndividual ,
                                                                      coy:CapitalControlsAndExchangeRatePolicy ;
                                                             rdfs:label "Controls on commercial transactions and investment instruments"@en .


###  https://schema.coypu.org/gta/ControlsOnCreditOperations
coy:ControlsOnCreditOperations rdf:type owl:NamedIndividual ,
                                        coy:CapitalControlsAndExchangeRatePolicy ;
                               rdfs:label "Controls on credit operations"@en .


###  https://schema.coypu.org/gta/ExportBan
coy:ExportBan rdf:type owl:NamedIndividual ,
                       coy:ExportAndImportPolicyInstruments ;
              rdfs:label "Export ban"@en .


###  https://schema.coypu.org/gta/ExportLicensingRequirement
coy:ExportLicensingRequirement rdf:type owl:NamedIndividual ,
                                        coy:ExportAndImportPolicyInstruments ;
                               rdfs:label "Export licensing requirement"@en .


###  https://schema.coypu.org/gta/ExportQuota
coy:ExportQuota rdf:type owl:NamedIndividual ,
                         coy:ExportAndImportPolicyInstruments ;
                rdfs:label "Export quota"@en .


###  https://schema.coypu.org/gta/ExportSubsidy
coy:ExportSubsidy rdf:type owl:NamedIndividual ,
                           coy:ExportAndImportPolicyInstruments ;
                  rdfs:label "Export subsidy"@en .


###  https://schema.coypu.org/gta/ExportTariffQuota
coy:ExportTariffQuota rdf:type owl:NamedIndividual ,
                               coy:ExportAndImportPolicyInstruments ;
                      rdfs:label "Export tariff quota"@en .


###  https://schema.coypu.org/gta/ExportTax
coy:ExportTax rdf:type owl:NamedIndividual ,
                       coy:ExportAndImportPolicyInstruments ;
              rdfs:label "Export tax"@en .


###  https://schema.coypu.org/gta/ExportTaxIncentive
coy:ExportTaxIncentive rdf:type owl:NamedIndividual ,
                                coy:ExportAndImportPolicyInstruments ;
                       rdfs:label "Export tax incentive"@en .


###  https://schema.coypu.org/gta/FinancialAssistanceInForeignMarket
coy:FinancialAssistanceInForeignMarket rdf:type owl:NamedIndividual ,
                                                coy:SubsidiesAndStateAid ;
                                       rdfs:label "Financial assistance in foreign market"@en .


###  https://schema.coypu.org/gta/FinancialGrant
coy:FinancialGrant rdf:type owl:NamedIndividual ,
                            coy:SubsidiesAndStateAid ;
                   rdfs:label "Financial grant"@en .


###  https://schema.coypu.org/gta/ForeignCustomerRule
coy:ForeignCustomerRule rdf:type owl:NamedIndividual ,
                                 coy:ExportAndImportPolicyInstruments ;
                        rdfs:label "Foreign customer rule"@en .


###  https://schema.coypu.org/gta/GreenTriangle
coy:GreenTriangle rdf:type owl:NamedIndividual ,
                           coy:GTAEvaluation ;
                  rdfs:comment "The intervention liberalises on a non-discriminatory (i.e., most favoured nation) basis; or improves the transparency of a relevant policy."@en ;
                  rdfs:label "green triangle"@en .


###  https://schema.coypu.org/gta/ImportBan
coy:ImportBan rdf:type owl:NamedIndividual ,
                       coy:ExportAndImportPolicyInstruments ;
              rdfs:label "Import ban"@en .


###  https://schema.coypu.org/gta/ImportIncentive
coy:ImportIncentive rdf:type owl:NamedIndividual ,
                             coy:ExportAndImportPolicyInstruments ;
                    rdfs:label "Import incentive"@en .


###  https://schema.coypu.org/gta/ImportLicensingRequirement
coy:ImportLicensingRequirement rdf:type owl:NamedIndividual ,
                                        coy:ExportAndImportPolicyInstruments ;
                               rdfs:label "Import licensing requirement"@en .


###  https://schema.coypu.org/gta/ImportMonitoring
coy:ImportMonitoring rdf:type owl:NamedIndividual ,
                              coy:ExportAndImportPolicyInstruments ;
                     rdfs:label "Import monitoring"@en .


###  https://schema.coypu.org/gta/ImportQuota
coy:ImportQuota rdf:type owl:NamedIndividual ,
                         coy:ExportAndImportPolicyInstruments ;
                rdfs:label "Import quota"@en .


###  https://schema.coypu.org/gta/ImportTariff
coy:ImportTariff rdf:type owl:NamedIndividual ,
                          coy:ExportAndImportPolicyInstruments ;
                 rdfs:label "Import tariff"@en .


###  https://schema.coypu.org/gta/ImportTariffQuota
coy:ImportTariffQuota rdf:type owl:NamedIndividual ,
                               coy:ExportAndImportPolicyInstruments ;
                      rdfs:label "Import tariff quota"@en .


###  https://schema.coypu.org/gta/In-kindGrant
coy:In-kindGrant rdf:type owl:NamedIndividual ,
                          coy:SubsidiesAndStateAid ;
                 rdfs:label "In-kind grant"@en .


###  https://schema.coypu.org/gta/IntellectualPropertyProtection
coy:IntellectualPropertyProtection rdf:type owl:NamedIndividual ,
                                            coy:OtherInstruments ;
                                   rdfs:label "Intellectual property protection"@en .


###  https://schema.coypu.org/gta/InterestPaymentSubsidy
coy:InterestPaymentSubsidy rdf:type owl:NamedIndividual ,
                                    coy:SubsidiesAndStateAid ;
                           rdfs:label "Interest payment subsidy"@en .


###  https://schema.coypu.org/gta/InternalTaxationOfImports
coy:InternalTaxationOfImports rdf:type owl:NamedIndividual ,
                                       coy:ExportAndImportPolicyInstruments ;
                              rdfs:label "Internal taxation of imports"@en .


###  https://schema.coypu.org/gta/Inward
coy:Inward rdf:type owl:NamedIndividual ,
                    coy:AffectedCommercialFlow ;
           rdfs:comment "The predominantly distorted market is the domestic market of the implementing jurisdiction."@en ;
           rdfs:label "Inward"@en .


###  https://schema.coypu.org/gta/LabourMarketAccess
coy:LabourMarketAccess rdf:type owl:NamedIndividual ,
                                coy:LaborForceMigrationPolicy ;
                       rdfs:label "Labour market access"@en .


###  https://schema.coypu.org/gta/LocalLabour
coy:LocalLabour rdf:type owl:NamedIndividual ,
                         coy:LocalisationPolicy ;
                rdfs:label "Local labour"@en .


###  https://schema.coypu.org/gta/LocalOperations
coy:LocalOperations rdf:type owl:NamedIndividual ,
                             coy:LocalisationPolicy ;
                    rdfs:label "Local operations"@en .


###  https://schema.coypu.org/gta/LocalSourcing
coy:LocalSourcing rdf:type owl:NamedIndividual ,
                           coy:LocalisationPolicy ,
                           coy:PublicProcurementPolicy ;
                  rdfs:label "Local sourcing"@en .


###  https://schema.coypu.org/gta/OtherExportInventive
coy:OtherExportInventive rdf:type owl:NamedIndividual ,
                                  coy:ExportAndImportPolicyInstruments ;
                         rdfs:label "Other export inventive"@en .


###  https://schema.coypu.org/gta/Outward
coy:Outward rdf:type owl:NamedIndividual ,
                     coy:AffectedCommercialFlow ;
            rdfs:comment "The documented change concerns an outflow restriction. The predominantly affected market is the outflow destination."@en ;
            rdfs:label "Outward"@en .


###  https://schema.coypu.org/gta/OutwardSubsidy
coy:OutwardSubsidy rdf:type owl:NamedIndividual ,
                            coy:AffectedCommercialFlow ;
                   rdfs:comment "In general, this value is only chosen for export incentives and trade finance interventions. In exceptional cases, a state aid awarded to an exporting company which generates its sales exclusively abroad may be classified as an outward subsidy."@en ;
                   rdfs:label "Outward subsidy"@en .


###  https://schema.coypu.org/gta/Post-migrationTreatment
coy:Post-migrationTreatment rdf:type owl:NamedIndividual ,
                                     coy:LaborForceMigrationPolicy ,
                                     coy:LocalisationPolicy ;
                            rdfs:label "Post-migration treatment"@en .


###  https://schema.coypu.org/gta/ProductionSubsidy
coy:ProductionSubsidy rdf:type owl:NamedIndividual ,
                               coy:SubsidiesAndStateAid ;
                      rdfs:label "Production subsidy"@en .


###  https://schema.coypu.org/gta/PublicProcurementAccess
coy:PublicProcurementAccess rdf:type owl:NamedIndividual ,
                                     coy:PublicProcurementPolicy ;
                            rdfs:label "Public procurement access"@en .


###  https://schema.coypu.org/gta/PublicProcurementLocalisation
coy:PublicProcurementLocalisation rdf:type owl:NamedIndividual ,
                                           coy:PublicProcurementPolicy ;
                                  rdfs:label "Public procurement localisation"@en .


###  https://schema.coypu.org/gta/PublicProcurementPreferenceMargin
coy:PublicProcurementPreferenceMargin rdf:type owl:NamedIndividual ,
                                               coy:PublicProcurementPolicy ;
                                      rdfs:label "Public procurement preference margin"@en .


###  https://schema.coypu.org/gta/RedTriangle
coy:RedTriangle rdf:type owl:NamedIndividual ,
                         coy:GTAEvaluation ;
                rdfs:comment "The intervention almost certainly discriminates against foreign commercial interests."@en ;
                rdfs:label "red triangle"@en .


###  https://schema.coypu.org/gta/Safeguard
coy:Safeguard rdf:type owl:NamedIndividual ,
                       coy:OtherInstruments ,
                       coy:TradeDefenceInstruments ;
              rdfs:label "Safeguard"@en .


###  https://schema.coypu.org/gta/SanitaryAndPhytosanitaryMeasure
coy:SanitaryAndPhytosanitaryMeasure rdf:type owl:NamedIndividual ,
                                             coy:OtherInstruments ;
                                    rdfs:label "Sanitary and phytosanitary measure"@en .


###  https://schema.coypu.org/gta/StateLoan
coy:StateLoan rdf:type owl:NamedIndividual ,
                       coy:SubsidiesAndStateAid ;
              rdfs:label "State loan"@en .


###  https://schema.coypu.org/gta/TaxOrSocialInsuranceRelief
coy:TaxOrSocialInsuranceRelief rdf:type owl:NamedIndividual ,
                                        coy:SubsidiesAndStateAid ;
                               rdfs:label "Tax or social insurance relief"@en .


###  https://schema.coypu.org/gta/TechnicalBarrierToTrade
coy:TechnicalBarrierToTrade rdf:type owl:NamedIndividual ,
                                     coy:OtherInstruments ;
                            rdfs:label "Technical barrier to trade"@en .


###  https://schema.coypu.org/gta/TradeBalancingMeasure
coy:TradeBalancingMeasure rdf:type owl:NamedIndividual ,
                                   coy:ExportAndImportPolicyInstruments ;
                          rdfs:label "Trade balancing measure"@en .


###  https://schema.coypu.org/gta/TradeFinance
coy:TradeFinance rdf:type owl:NamedIndividual ,
                          coy:ExportAndImportPolicyInstruments ;
                 rdfs:label "Trade finance"@en .


###  https://schema.coypu.org/gta/TradePaymentMeasure
coy:TradePaymentMeasure rdf:type owl:NamedIndividual ,
                                 coy:ExportAndImportPolicyInstruments ,
                                 coy:ForeignInvestmentPolicy ;
                        rdfs:label "Trade payment measure"@en .


###  https://schema.coypu.org/gta/Bailout%28CapitalInjectionOrEquityParticipation%29
<https://schema.coypu.org/gta/Bailout%28CapitalInjectionOrEquityParticipation%29> rdf:type owl:NamedIndividual ,
                                                                                           coy:SubsidiesAndStateAid ;
                                                                                  rdfs:label "Bailout (capital injection or equity participation)"@en .


###  https://schema.coypu.org/gta/Export-relatedNon-TariffMeasure%2CNes
<https://schema.coypu.org/gta/Export-relatedNon-TariffMeasure%2CNes> rdf:type owl:NamedIndividual ,
                                                                              coy:ExportAndImportPolicyInstruments ;
                                                                     rdfs:label "Export-related non-tariff measure, nes"@en .


###  https://schema.coypu.org/gta/FDI%3AEntryAndOwnershipRule
<https://schema.coypu.org/gta/FDI%3AEntryAndOwnershipRule> rdf:type owl:NamedIndividual ,
                                                                    coy:ForeignInvestmentPolicy ;
                                                           rdfs:label "FDI: Entry and ownership rule"@en .


###  https://schema.coypu.org/gta/FDI%3AFinancialIncentive
<https://schema.coypu.org/gta/FDI%3AFinancialIncentive> rdf:type owl:NamedIndividual ,
                                                                 coy:ForeignInvestmentPolicy ;
                                                        rdfs:label "FDI: Financial incentive"@en .


###  https://schema.coypu.org/gta/FDI%3ATreatmentAndOperations%2CNes
<https://schema.coypu.org/gta/FDI%3ATreatmentAndOperations%2CNes> rdf:type owl:NamedIndividual ,
                                                                           coy:ForeignInvestmentPolicy ,
                                                                           coy:LaborForceMigrationPolicy ;
                                                                  rdfs:label "FDI: Treatment and operations, nes"@en .


###  https://schema.coypu.org/gta/Import-relatedNon-TariffMeasure%2CNes
<https://schema.coypu.org/gta/Import-relatedNon-TariffMeasure%2CNes> rdf:type owl:NamedIndividual ,
                                                                              coy:ExportAndImportPolicyInstruments ;
                                                                     rdfs:label "Import-related non-tariff measure, nes"@en .


###  https://schema.coypu.org/gta/PublicProcurement%2CNes
<https://schema.coypu.org/gta/PublicProcurement%2CNes> rdf:type owl:NamedIndividual ,
                                                                coy:PublicProcurementPolicy ,
                                                                coy:SubsidiesAndStateAid ;
                                                       rdfs:label "Public procurement, nes"@en .


###  https://schema.coypu.org/gta/Repatriation%26SurrenderRequirements
<https://schema.coypu.org/gta/Repatriation%26SurrenderRequirements> rdf:type owl:NamedIndividual ,
                                                                             coy:CapitalControlsAndExchangeRatePolicy ;
                                                                    rdfs:label "Repatriation & surrender requirements"@en .


###  https://schema.coypu.org/gta/StateAid%2CNes
<https://schema.coypu.org/gta/StateAid%2CNes> rdf:type owl:NamedIndividual ,
                                                       coy:SubsidiesAndStateAid ,
                                                       coy:TradeDefenceInstruments ;
                                              rdfs:label "State aid, nes"@en .


###  https://schema.coypu.org/gta/TradePaymentMeasure%28SeeExportAndImportSection%29
<https://schema.coypu.org/gta/TradePaymentMeasure%28SeeExportAndImportSection%29> rdf:type owl:NamedIndividual ,
                                                                                           coy:CapitalControlsAndExchangeRatePolicy ,
                                                                                           coy:ExportAndImportPolicyInstruments ;
                                                                                  rdfs:label "Trade payment measure (see export and import section)"@en .


###  Generated by the OWL API (version 4.5.9.2019-02-01T07:24:44Z) https://github.com/owlcs/owlapi
