@prefix : <https://schema.coypu.org/tiva#> .
@prefix coy: <https://schema.coypu.org/global#> .
@prefix owl: <http://www.w3.org/2002/07/owl#> .
@prefix rdf: <http://www.w3.org/1999/02/22-rdf-syntax-ns#> .
@prefix xml: <http://www.w3.org/XML/1998/namespace> .
@prefix xsd: <http://www.w3.org/2001/XMLSchema#> .
@prefix rdfs: <http://www.w3.org/2000/01/rdf-schema#> .
@prefix tiva: <https://schema.coypu.org/tiva#> .
@prefix dcterms: <http://purl.org/dc/terms/> .
@base <https://schema.coypu.org/tiva> .

<https://schema.coypu.org/tiva> rdf:type owl:Ontology ;
                                 owl:versionIRI <https://schema.coypu.org/tiva/1.4> ;
                                 dcterms:contributor "Felix Engel"@en ,
                                                     "Nenad Krdzavac"@en ,
                                                     "Nils Steinert"@en ;
                                 rdfs:comment "An ontology for modeling international trade flows."@en ;
                                 rdfs:label "OECD TIVA Ontology"@en ;
                                 owl:versionInfo 1.4 .

#################################################################
#    Annotation properties
#################################################################

###  http://purl.org/dc/terms/contributor
dcterms:contributor rdf:type owl:AnnotationProperty .


#################################################################
#    Object Properties
#################################################################

###  https://schema.coypu.org/tiva#hasExport
tiva:hasExport rdf:type owl:ObjectProperty ;
               rdfs:range tiva:Export ;
               rdfs:label "has export"@en .


###  https://schema.coypu.org/tiva#hasFinalDemand
tiva:hasFinalDemand rdf:type owl:ObjectProperty ;
                    rdfs:range tiva:Fd ;
                    rdfs:label "has final demand"@en .


###  https://schema.coypu.org/tiva#hasImport
tiva:hasImport rdf:type owl:ObjectProperty ;
               rdfs:range tiva:Import ;
               rdfs:label "has import"@en .


###  https://schema.coypu.org/tiva#hasIndustryCode
tiva:hasIndustryCode rdf:type owl:ObjectProperty ;
                     rdfs:range <https://spec.edmcouncil.org/fibo/ontology/FND/Arrangements/ClassificationSchemes/IndustrySectorClassificationScheme> ;
                     rdfs:label "has industry code"@en .


###  https://schema.coypu.org/tiva#hasValueAddedOrigin
tiva:hasValueAddedOrigin rdf:type owl:ObjectProperty ;
                         rdfs:range tiva:Vao ;
                         rdfs:label "has value added origin"@en .


#################################################################
#    Classes
#################################################################

###  https://schema.coypu.org/tiva#ExgrBsci
tiva:ExgrBsci rdf:type owl:Class ;
              rdfs:subClassOf tiva:TradeInValueAdded ;
              rdfs:comment "Origin of value added in gross exports provides estimates of total gross exports by exporting industry I in country C broken down by the value added generated by source industry H in country P."@en ;
              rdfs:label "OriginOfValueAddedGrossExports"@en ;
              rdfs:seeAlso "https://stats.oecd.org/fileview2.aspx?IDFile=eefca001-71ab-497e-9abd-5e0c58c27ed4" .


###  https://schema.coypu.org/tiva#Export
tiva:Export rdf:type owl:Class ;
            rdfs:subClassOf tiva:TradeInValueAdded ;
            rdfs:comment "Presents gross exports of final products by industry I in country C, broken down by both the source country/region S origin of value added and according to final demand destination country/region P."@en ;
            rdfs:label "Exports"@en .


###  https://schema.coypu.org/tiva#Fd
tiva:Fd rdf:type owl:Class ;
        rdfs:subClassOf tiva:TradeInValueAdded ;
        rdfs:comment """Domestic Final Demand (DFD): A measure of spending. Specifically, the sum of final consumption, investment and stock building expenditures, by both private and government sectors

State Final Demand (SFD): State Final Demand measures the total value of goods and services that are sold in a state to buyers (who wish to consume them or retain them in the form of Capital Assets). SFD is the state-level equivalent of DFD."""@en ;
        rdfs:label "FinalDemand"@en ;
        rdfs:seeAlso "https://www.treasury.sa.gov.au/economy,-taxes-and-rebates/economic-briefs/glossary#:~:text=Domestic%20Final%20Demand%20(DFD),both%20private%20and%20government%20sectors." .


###  https://schema.coypu.org/tiva#FdExgrVa
tiva:FdExgrVa rdf:type owl:Class ;
              rdfs:subClassOf tiva:TradeInValueAdded ;
              rdfs:comment "This indicator (FD_EXGR_VA) presents gross exports of final and intermediate products by industry I in country C, broken down by both the source country/region s origin of value  added and, according to final demand destination country/region P."@en ;
              rdfs:label "GrossExports"@en ;
              rdfs:seeAlso "https://stats.oecd.org/fileview2.aspx?IDFile=eefca001-71ab-497e-9abd-5e0c58c27ed4" .


###  https://schema.coypu.org/tiva#FdVaBsci
tiva:FdVaBsci rdf:type owl:Class ;
              rdfs:subClassOf tiva:TradeInValueAdded ;
              rdfs:comment "Origin of value added in final demand provides estimates of value added for final demand in country P for industry H for final goods and services broken down by the value added generated by source industry I in VA source country C."@en ;
              rdfs:label "OriginOfValueAddedFinalDemand"@en ;
              rdfs:seeAlso "https://stats.oecd.org/fileview2.aspx?IDFile=eefca001-71ab-497e-9abd-5e0c58c27ed4" .


###  https://schema.coypu.org/tiva#ImgrBsci
tiva:ImgrBsci rdf:type owl:Class ;
              rdfs:subClassOf tiva:TradeInValueAdded ;
              rdfs:comment "Origin of value added in gross imports provides estimates of the value added in gross imports by country C of goods and services from industry I originating from partner country/region P broken down by value added originating from country/region S."@en ;
              rdfs:label "OriginOfValueAddedGrossImports"@en ;
              rdfs:seeAlso "https://stats.oecd.org/fileview2.aspx?IDFile=eefca001-71ab-497e-9abd-5e0c58c27ed4" .


###  https://schema.coypu.org/tiva#Import
tiva:Import rdf:type owl:Class ;
            rdfs:subClassOf tiva:TradeInValueAdded ;
            rdfs:comment "Domestic value added content of gross imports reveals the value added generated in country C that returns to country C embodied in gross imports from industry I in partner country P."@en ;
            rdfs:label "Imports"@en ;
            rdfs:seeAlso "https://stats.oecd.org/fileview2.aspx?IDFile=eefca001-71ab-497e-9abd-5e0c58c27ed4" .


###  https://schema.coypu.org/tiva#Isic
tiva:Isic rdf:type owl:Class ;
          rdfs:subClassOf <https://spec.edmcouncil.org/fibo/ontology/FND/Arrangements/ClassificationSchemes/IndustrySectorClassificationScheme> ;
          rdfs:comment "International standard industrial classification of all economic activities (ISIC), Rev. 4."@en ;
          rdfs:label "ISIC4" ;
          rdfs:seeAlso "https://unstats.un.org/unsd/publication/seriesm/seriesm_4rev4e.pdf" .


###  https://schema.coypu.org/tiva#TradeInValueAdded
tiva:TradeInValueAdded rdf:type owl:Class .


###  https://schema.coypu.org/tiva#Vao
tiva:Vao rdf:type owl:Class ;
         rdfs:subClassOf tiva:TradeInValueAdded ;
         rdfs:comment "Domestic value added origin is shown where source country P=C, additionally represented by source country = “DXD: Domestic”."@en ;
         rdfs:label "ValueAddedOrigin"@en ;
         rdfs:seeAlso "https://stats.oecd.org/fileview2.aspx?IDFile=eefca001-71ab-497e-9abd-5e0c58c27ed4" .


###  https://spec.edmcouncil.org/fibo/ontology/FND/Arrangements/ClassificationSchemes/IndustrySectorClassificationScheme
<https://spec.edmcouncil.org/fibo/ontology/FND/Arrangements/ClassificationSchemes/IndustrySectorClassificationScheme> rdf:type owl:Class ;
                                                                                                                      rdfs:subClassOf tiva:TradeInValueAdded ;
                                                                                                                      rdfs:label "SectorClassificationScheme"@en .


###  Generated by the OWL API (version 4.5.9.2019-02-01T07:24:44Z) https://github.com/owlcs/owlapi
